HelpingOnOffproof + HelpingFacts Complete

helping/HelpingAux.v
@@ -4,7 +4,7 @@ Require Import GSim GSimFacts GSimTactics.
 Require Import SchHeader SchI SchA.
 From CRIS.helping Require Import Header HelpingOn HelpingOff.
 
-
+(* This file contains auxilliary lemmas for proving HelpOn ≼ HelpOff. *)
 Section auxilliary.
 
   Context {Σ : GRA}.
@@ -28,153 +28,154 @@ Section auxilliary.
 
 End auxilliary.
 
-  Tactic Notation "red_bind" tactic(tac) :=
-    lazymatch goal with
-    | [ |- @ITree.bind _ _ _ ?itr _ = _ ] =>
-        lazymatch itr with
-        | Ret _ => etransitivity; [ eapply bind_ret_l | s; tac ]
-        | Tau _ => eapply bind_tau
-        | vis _ _ => eapply vis_bind
-        | assumeK _ _ => eapply assumeK_bind
-        | guaranteeK _ _ => eapply guaranteeK_bind
-        | unwrapUK _ _ => eapply unwrapUK_bind
-        | unwrapNK _ _ => eapply unwrapNK_bind
-        | RealUpdateK _ _ => eapply RealUpdateK_bind
-        | SBRed.putSB _ _ _ _ _ _ => eapply SBRed.putSB_bind
-        | SBRed.getSB _ _ _ _ _ => eapply SBRed.getSB_bind
-        | SBRed.callSB _ _ _ _ _ _ => eapply SBRed.callSB_bind
-        | SBRed.spawnSB _ _ _ _ _ _ => eapply SBRed.spawnSB_bind
-        | @ITree.bind _ _ _ _ _ => eapply bind_bind
-        | _ => reflexivity
-        end
-    end.
-
-  Tactic Notation "red_SB" :=
-    lazymatch goal with
-    | [ |- @SB.sandbox _ _ _ _ _ ?itr = _ ] =>
-        lazymatch itr with
-        | Ret _ =>
-            eapply SBRed.ret
-        | Tau _ =>
-            eapply SBRed.tau
-        | vis (Assume _) _ =>
-            first [eapply SBRed.vis_Assume_img|eapply SBRed.vis_Assume]
-        | vis (AssumeRes _) _ =>
-            eapply SBRed.vis_AssumeRes
-        | vis (Guarantee _) _ =>
-            eapply SBRed.vis_Guarantee
-        | vis (Spawn _ _) _ =>
-            eapply SBRed.Spawn_spawnSB
-        | vis (Yield _) _ =>
-            eapply SBRed.vis_yield
-        | vis (Call _ _) _ =>
-            eapply SBRed.Call_callSB
-        | vis (SPut _ _) _ =>
-            eapply SBRed.SPut_putSB
-        | vis (SGet _) _ =>
-            eapply SBRed.SGet_getSB
-        | vis (Choose _) _ =>
-            eapply SBRed.vis_choose
-        | vis (Take _) _ =>
-            first [eapply SBRed.vis_take_img|eapply SBRed.vis_take]
-        | vis (IO _ _) _ =>
-            eapply SBRed.vis_io
-        | assumeK _ _ =>
-            eapply SBRed.assumeK
-        | guaranteeK _ _ =>
-            eapply SBRed.guaranteeK
-        | unwrapUK _ _ =>
-            eapply SBRed.unwrapUK
-        | unwrapNK _ _ =>
-            eapply SBRed.unwrapNK
-        | RealUpdateK _ _ _ =>
-            eapply SBRed.ruK
-        | @ITree.bind _ _ _ _ _ =>
-            eapply SBRed.bind
-        | _ =>
-            reflexivity
-        end
-    end.
-
-  Tactic Notation "red_S" tactic(tac) :=
-    lazymatch goal with
-    | [ |- @SModTr.trans _ ?sp _ ?itr = _ ] =>
-        lazymatch itr with
-        | Ret _ =>
-            eapply SRed.ret
-        | Tau _ =>
-            eapply SRed.tau
-        | vis (Assume _) _ =>
-            eapply SRed.vis_ag
-        | vis (AssumeRes _) _ =>
-            eapply SRed.vis_ag
-        | vis (Guarantee _) _ =>
-            eapply SRed.vis_ag
-        | vis (Spawn ?fn _) _ =>
-            etransitivity;
-            [ eapply SRed.vis_spawn
-            | unfold SModTr.HoareSpawn, SModTr.NativeSpawn;
-              unfold_sp_exact sp fn; s;
-              tac
-            ]
-        | vis (Yield _) _ =>
-            etransitivity;
-            [ eapply SRed.vis_yield
-            | tac
-            ]
-        | vis (Call ?fn _) _ =>
-            etransitivity;
-            [ eapply SRed.vis_call
-            | unfold SModTr.HoareCall;
-              unfold_sp_exact sp fn; s;
-              tac
-            ]
-        | vis (SPut _ _) _ =>
-            eapply SRed.vis_pg
-        | vis (SGet _) _ =>
-            eapply SRed.vis_pg
-        | vis (Choose _) _ =>
-            eapply SRed.vis_core
-        | vis (Take _) _ =>
-            eapply SRed.vis_core
-        | vis (IO _ _) _ =>
-            eapply SRed.vis_core
-        | assumeK _ _ =>
-            eapply SRed.assumeK
-        | guaranteeK _ _ =>
-            eapply SRed.guaranteeK
-        | unwrapUK _ _ =>
-            eapply SRed.unwrapUK
-        | unwrapNK _ _ =>
-            eapply SRed.unwrapNK
-        | RealUpdateK _ _ _ =>
-            eapply SRed.ruK
-        | @ITree.bind _ _ _ _ _ =>
-            eapply SRed.bind
-        | _ =>
-            reflexivity
-        end
-    end.
-
-  Ltac replace_l :=
-    match goal with
-    | |- gpaco7 _ _ _ _ _ _ _ _ _ ?itr _ =>
-      pattern itr;
-      match goal with
-      | |- ?f ?a =>
-        refine (eq_ind_r f _ _); cycle 1
+Tactic Notation "red_bind" tactic(tac) :=
+  lazymatch goal with
+  | [ |- @ITree.bind _ _ _ ?itr _ = _ ] =>
+      lazymatch itr with
+      | Ret _ => etransitivity; [ eapply bind_ret_l | s; tac ]
+      | Tau _ => eapply bind_tau
+      | vis _ _ => eapply vis_bind
+      | assumeK _ _ => eapply assumeK_bind
+      | guaranteeK _ _ => eapply guaranteeK_bind
+      | unwrapUK _ _ => eapply unwrapUK_bind
+      | unwrapNK _ _ => eapply unwrapNK_bind
+      | RealUpdateK _ _ => eapply RealUpdateK_bind
+      | SBRed.putSB _ _ _ _ _ _ => eapply SBRed.putSB_bind
+      | SBRed.getSB _ _ _ _ _ => eapply SBRed.getSB_bind
+      | SBRed.callSB _ _ _ _ _ _ => eapply SBRed.callSB_bind
+      | SBRed.spawnSB _ _ _ _ _ _ => eapply SBRed.spawnSB_bind
+      | @ITree.bind _ _ _ _ _ => eapply bind_bind
+      | _ => reflexivity
       end
-    end.
+  end.
 
-  Ltac replace_r :=
-    match goal with
-    | |- gpaco7 _ _ _ _ _ _ _ _ _ _ ?itr =>
-      pattern itr;
-      match goal with
-      | |- ?f ?a =>
-        refine (eq_ind_r f _ _); cycle 1
+Tactic Notation "red_SB" :=
+  lazymatch goal with
+  | [ |- @SB.sandbox _ _ _ _ _ ?itr = _ ] =>
+      lazymatch itr with
+      | Ret _ =>
+          eapply SBRed.ret
+      | Tau _ =>
+          eapply SBRed.tau
+      | vis (Assume _) _ =>
+          first [eapply SBRed.vis_Assume_img|eapply SBRed.vis_Assume]
+      | vis (AssumeRes _) _ =>
+          eapply SBRed.vis_AssumeRes
+      | vis (Guarantee _) _ =>
+          eapply SBRed.vis_Guarantee
+      | vis (Spawn _ _) _ =>
+          eapply SBRed.Spawn_spawnSB
+      | vis (Yield _) _ =>
+          eapply SBRed.vis_yield
+      | vis (Call _ _) _ =>
+          eapply SBRed.Call_callSB
+      | vis (SPut _ _) _ =>
+          eapply SBRed.SPut_putSB
+      | vis (SGet _) _ =>
+          eapply SBRed.SGet_getSB
+      | vis (Choose _) _ =>
+          eapply SBRed.vis_choose
+      | vis (Take _) _ =>
+          first [eapply SBRed.vis_take_img|eapply SBRed.vis_take]
+      | vis (IO _ _) _ =>
+          eapply SBRed.vis_io
+      | assumeK _ _ =>
+          eapply SBRed.assumeK
+      | guaranteeK _ _ =>
+          eapply SBRed.guaranteeK
+      | unwrapUK _ _ =>
+          eapply SBRed.unwrapUK
+      | unwrapNK _ _ =>
+          eapply SBRed.unwrapNK
+      | RealUpdateK _ _ _ =>
+          eapply SBRed.ruK
+      | @ITree.bind _ _ _ _ _ =>
+          eapply SBRed.bind
+      | _ =>
+          reflexivity
       end
-    end.
+  end.
+
+Tactic Notation "red_S" tactic(tac) :=
+  lazymatch goal with
+  | [ |- @SModTr.trans _ ?sp _ ?itr = _ ] =>
+      lazymatch itr with
+      | Ret _ =>
+          eapply SRed.ret
+      | Tau _ =>
+          eapply SRed.tau
+      | vis (Assume _) _ =>
+          eapply SRed.vis_ag
+      | vis (AssumeRes _) _ =>
+          eapply SRed.vis_ag
+      | vis (Guarantee _) _ =>
+          eapply SRed.vis_ag
+      | vis (Spawn ?fn _) _ =>
+          etransitivity;
+          [ eapply SRed.vis_spawn
+          | unfold SModTr.HoareSpawn, SModTr.NativeSpawn;
+            unfold_sp_exact sp fn; s;
+            tac
+          ]
+      | vis (Yield _) _ =>
+          etransitivity;
+          [ eapply SRed.vis_yield
+          | tac
+          ]
+      | vis (Call ?fn _) _ =>
+          etransitivity;
+          [ eapply SRed.vis_call
+          | unfold SModTr.HoareCall;
+            unfold_sp_exact sp fn; s;
+            tac
+          ]
+      | vis (SPut _ _) _ =>
+          eapply SRed.vis_pg
+      | vis (SGet _) _ =>
+          eapply SRed.vis_pg
+      | vis (Choose _) _ =>
+          eapply SRed.vis_core
+      | vis (Take _) _ =>
+          eapply SRed.vis_core
+      | vis (IO _ _) _ =>
+          eapply SRed.vis_core
+      | assumeK _ _ =>
+          eapply SRed.assumeK
+      | guaranteeK _ _ =>
+          eapply SRed.guaranteeK
+      | unwrapUK _ _ =>
+          eapply SRed.unwrapUK
+      | unwrapNK _ _ =>
+          eapply SRed.unwrapNK
+      | RealUpdateK _ _ _ =>
+          eapply SRed.ruK
+      | @ITree.bind _ _ _ _ _ =>
+          eapply SRed.bind
+      | _ =>
+          reflexivity
+      end
+  end.
+
+Ltac replace_l :=
+  match goal with
+  | |- gpaco7 _ _ _ _ _ _ _ _ _ ?itr _ =>
+    pattern itr;
+    match goal with
+    | |- ?f ?a =>
+      refine (eq_ind_r f _ _); cycle 1
+    end
+  end.
+
+Ltac replace_r :=
+  match goal with
+  | |- gpaco7 _ _ _ _ _ _ _ _ _ _ ?itr =>
+    pattern itr;
+    match goal with
+    | |- ?f ?a =>
+      refine (eq_ind_r f _ _); cycle 1
+    end
+  end.
+
 Tactic Notation "red_LModTr" tactic(tac) :=
   match goal with
   | |- ?H => idtac H
@@ -240,188 +241,186 @@ Tactic Notation "red_ModTr" tactic(tac) :=
       end
   end.
 
-  (* Local Lemma LModTr_interp_stateE_bind {A B} itr state : *)
-    
-  Tactic Notation "red_LModTr_state" tactic(tac) :=
-    lazymatch goal with
-    | [ |- @LModTr.interp_stateE ?A ?B ?itr ?state = _] =>
-      match itr with
-      | @iterV ?A ?B ?C ?handle ?itr => reflexivity
-      | _ =>
-        etransitivity;
-        [rewrite /= /LModTr.interp_stateE;
-          lazymatch itr with
-          | @ITree.bind _ _ _ _ _ =>
-            eapply interp_state_bind
-          | Ret _ =>
-            eapply interp_state_ret
-          | vis _ _ =>
-            etransitivity; [eapply interp_state_vis|tac; refl]
-          | Tau _ =>
-            eapply interp_state_tau
-          | unwrapUK _ _ =>
-            etransitivity; [rewrite /unwrapUK; refl|tac]
-          | _ =>
-            reflexivity
-          end
-        | fold (@LModTr.interp_stateE coreE); refl]
-      end
-    end.
-
-  Ltac _gnorm_itr :=
-    lazymatch goal with
-    | [ |- Ret _ = _ ] =>
-        reflexivity
-    | [ |- Tau _ = _ ] =>
-        reflexivity
-    | [ |- vis _ _ = _ ] =>
-        reflexivity
-    | [ |- @ITree.bind ?E ?T ?U ?itr ?ktr = _ ] =>
-        etransitivity;
-        [ let itr' := fresh "itr" in cong (fun (itr' : itree E T) => @ITree.bind E T U itr' ktr); _gnorm_itr
-        | s; red_bind (do 1 _gnorm_itr) ]
-    | [ |- @SB.sandbox ?Σ ?R ?img ?imports ?scopes ?itr = _ ] =>
-        etransitivity;
-        [ cong (@SB.sandbox Σ R img imports scopes); _gnorm_itr | red_SB ]
-    | [ |- @SModTr.trans ?Σ ?sp ?R ?itr = _ ] =>
-        etransitivity;
-        [ cong (@SModTr.trans Σ sp R); _gnorm_itr | red_S (do 1 _gnorm_itr) ]
-    | [ |- @LModTr.interp_stateE ?E ?T ?itr ?st = _] =>
-        etransitivity;
-        [ cong (λ i, @LModTr.interp_stateE E T i st); _gnorm_itr | red_LModTr_state (do 1 _gnorm_itr)]
-    (* | [ |- @iterV ?A ?B ?C ?handle ?itr = _ ] =>
-        idtac "iterV "; idtac itr;
-        (rewrite unfold_iterV /itreeV_itree;
-        lazymatch goal with
-        | |- context [@LModTr.handle_callE ?A ?B] =>
-          pattern (LModTr.handle_callE A B);
-          lazymatch goal with
-          | [ |- ?f ?a] =>
-            refine (eq_ind_r f _ _); cycle 1;
-            [_gnorm_itr
-            | lazymatch goal with
-              | |- context [_observe ?f] => idtac f; fail
-              | |- _ => s; _gnorm_itr
-              end
-            ]
-          end
+Tactic Notation "red_LModTr_state" tactic(tac) :=
+  lazymatch goal with
+  | [ |- @LModTr.interp_stateE ?A ?B ?itr ?state = _] =>
+    match itr with
+    | @iterV ?A ?B ?C ?handle ?itr => reflexivity
+    | _ =>
+      etransitivity;
+      [rewrite /= /LModTr.interp_stateE;
+        lazymatch itr with
+        | @ITree.bind _ _ _ _ _ =>
+          eapply interp_state_bind
+        | Ret _ =>
+          eapply interp_state_ret
+        | vis _ _ =>
+          etransitivity; [eapply interp_state_vis|tac; refl]
+        | Tau _ =>
+          eapply interp_state_tau
+        | unwrapUK _ _ =>
+          etransitivity; [rewrite /unwrapUK; refl|tac]
+        | _ =>
+          reflexivity
         end
-        + refl) *)
-    | [ |- @case_ _ _ _ _ _ _ _ _ _ _ _ ?E = _] =>
-        rewrite /case_ /LModTr.pure_state /=; _gnorm_itr
-    | [ |- @ModTr.trans ?A ?B ?itr = _] =>
-        etransitivity;
-        [ cong (@ModTr.trans A B); _gnorm_itr | red_ModTr (do 1 _gnorm_itr) ]
-    | [ |- @LModTr.handle_callE ?prog ?a = _] =>
-      rewrite /LModTr.handle_callE;
-      match goal with
-      | |- context [?a !! ?b] =>
-        pattern (a !! b);
-        match goal with
-        | |- ?f ?a =>
-          eapply (eq_ind_r f); cycle 1; [s; eapply (f_equal Some); _gnorm_itr|ss]
-        end
-      end
-    | [ |- trigger _ = _ ] =>
-        eapply trigger_vis
-    | [ |- assume _ = _ ] =>
-        eapply assume_assumeK
-    | [ |- guarantee _ = _ ] =>
-        eapply guarantee_guaranteeK
-    | [ |- unwrapU _ = _ ] =>
-        eapply unwrapU_unwrapUK
-    | [ |- unwrapN _ = _ ] =>
-        eapply unwrapN_unwrapNK
-    | [ |- RealUpdate _ _ = _ ] =>
-        eapply RealUpdate_RealUpdateK
-    | [ |- SModTr.HoareCall _ _ _ = _ ] =>
-        unfold SModTr.HoareCall;
-        _gnorm_itr
-    | [ |- SModTr.NativeSpawn _ _ = _ ] =>
-        unfold SModTr.NativeSpawn;
-        _gnorm_itr
-    | [ |- fbody_trivial _ = _ ] =>
-        unfold fbody_trivial;
-        _gnorm_itr
-    | [ |- cput _ _ = _ ] =>
-        unfold cput;
-        _gnorm_itr
-    | [ |- cgetU _ = _ ] =>
-        unfold cgetU;
-        _gnorm_itr
-    | [ |- cgetN _ = _ ] =>
-        unfold cgetN;
-        _gnorm_itr
-    | [ |- cfunU _ _ = _ ] =>
-        unfold cfunU;
-        _gnorm_itr
-    | [ |- cfunN _ _ = _ ] =>
-        unfold cfunN;
-        _gnorm_itr
-    | [ |- ccallU _ _ = _ ] =>
-        unfold ccallU;
-        _gnorm_itr
-    | [ |- ccallN _ _ = _ ] =>
-        unfold ccallN;
-        _gnorm_itr
-    | [ |- triggerUB = _ ] =>
-        unfold triggerUB;
-        _gnorm_itr
-    | [ |- triggerNB = _ ] =>
-        unfold triggerNB;
-        _gnorm_itr
-    | [ |- ?itr = _ ] =>
-        reflexivity
-  end.
-  Ltac gnorm_itr :=
-  etransitivity;
-  [ _gnorm_itr
-  | s;
-    lazymatch goal with
-    | [ |- Ret _ = _ ] =>
-        reflexivity
-    | [ |- Tau _ = _ ] =>
-        reflexivity
-    | [ |- vis _ _ = _ ] =>
-        eapply vis_trigger
-    | [ |- _ = _ ] =>
-        reflexivity
+      | fold (@LModTr.interp_stateE coreE); refl]
     end
-  ].
+  end.
 
-  Ltac norm_l :=
-    replace_l; [s; gnorm_itr|].
-  Ltac norm_r :=
-    replace_r; [s; gnorm_itr|].
-
-  Ltac iter_l :=
-    replace_l; [rewrite unfold_iterV /itreeV_itree //|]; norm_l.
-  Ltac iter_r :=
-    replace_r; [rewrite unfold_iterV /itreeV_itree //|]; norm_r.
-
-  Ltac step_r :=
-    norm_r; guclo gsim_indC_spec; econs; instantiate (1:=smj_top).
-  Ltac step_l :=
-    norm_l; guclo gsim_indC_spec; econs; instantiate (1:=smj_top).
-
-  Ltac replace_tp_r :=
-    match goal with
-    | |- gpaco7 _ _ _ _ _ _ _ _ _ _ (LModTr.interp_stateE _ (iterV _ ?tp) _) =>
-        pattern tp;
-        match goal with
-        | |- ?f ?tp =>
-            eapply (eq_ind_r f); cycle 1
+Ltac _gnorm_itr :=
+  lazymatch goal with
+  | [ |- Ret _ = _ ] =>
+      reflexivity
+  | [ |- Tau _ = _ ] =>
+      reflexivity
+  | [ |- vis _ _ = _ ] =>
+      reflexivity
+  | [ |- @ITree.bind ?E ?T ?U ?itr ?ktr = _ ] =>
+      etransitivity;
+      [ let itr' := fresh "itr" in cong (fun (itr' : itree E T) => @ITree.bind E T U itr' ktr); _gnorm_itr
+      | s; red_bind (do 1 _gnorm_itr) ]
+  | [ |- @SB.sandbox ?Σ ?R ?img ?imports ?scopes ?itr = _ ] =>
+      etransitivity;
+      [ cong (@SB.sandbox Σ R img imports scopes); _gnorm_itr | red_SB ]
+  | [ |- @SModTr.trans ?Σ ?sp ?R ?itr = _ ] =>
+      etransitivity;
+      [ cong (@SModTr.trans Σ sp R); _gnorm_itr | red_S (do 1 _gnorm_itr) ]
+  | [ |- @LModTr.interp_stateE ?E ?T ?itr ?st = _] =>
+      etransitivity;
+      [ cong (λ i, @LModTr.interp_stateE E T i st); _gnorm_itr | red_LModTr_state (do 1 _gnorm_itr)]
+  (* | [ |- @iterV ?A ?B ?C ?handle ?itr = _ ] =>
+      idtac "iterV "; idtac itr;
+      (rewrite unfold_iterV /itreeV_itree;
+      lazymatch goal with
+      | |- context [@LModTr.handle_callE ?A ?B] =>
+        pattern (LModTr.handle_callE A B);
+        lazymatch goal with
+        | [ |- ?f ?a] =>
+          refine (eq_ind_r f _ _); cycle 1;
+          [_gnorm_itr
+          | lazymatch goal with
+            | |- context [_observe ?f] => idtac f; fail
+            | |- _ => s; _gnorm_itr
+            end
+          ]
         end
-    end.
-  Ltac replace_tp_l :=
+      end
+      + refl) *)
+  | [ |- @case_ _ _ _ _ _ _ _ _ _ _ _ ?E = _] =>
+      rewrite /case_ /LModTr.pure_state /=; _gnorm_itr
+  | [ |- @ModTr.trans ?A ?B ?itr = _] =>
+      etransitivity;
+      [ cong (@ModTr.trans A B); _gnorm_itr | red_ModTr (do 1 _gnorm_itr) ]
+  | [ |- @LModTr.handle_callE ?prog ?a = _] =>
+    rewrite /LModTr.handle_callE;
     match goal with
-    | |- gpaco7 _ _ _ _ _ _ _ _ _ (LModTr.interp_stateE _ (iterV _ ?tp) _) _ =>
-        pattern tp;
-        match goal with
-        | |- ?f ?tp =>
-            eapply (eq_ind_r f); cycle 1
-        end
-    end.
+    | |- context [?a !! ?b] =>
+      pattern (a !! b);
+      match goal with
+      | |- ?f ?a =>
+        eapply (eq_ind_r f); cycle 1; [s; eapply (f_equal Some); _gnorm_itr|ss]
+      end
+    end
+  | [ |- trigger _ = _ ] =>
+      eapply trigger_vis
+  | [ |- assume _ = _ ] =>
+      eapply assume_assumeK
+  | [ |- guarantee _ = _ ] =>
+      eapply guarantee_guaranteeK
+  | [ |- unwrapU _ = _ ] =>
+      eapply unwrapU_unwrapUK
+  | [ |- unwrapN _ = _ ] =>
+      eapply unwrapN_unwrapNK
+  | [ |- RealUpdate _ _ = _ ] =>
+      eapply RealUpdate_RealUpdateK
+  | [ |- SModTr.HoareCall _ _ _ = _ ] =>
+      unfold SModTr.HoareCall;
+      _gnorm_itr
+  | [ |- SModTr.NativeSpawn _ _ = _ ] =>
+      unfold SModTr.NativeSpawn;
+      _gnorm_itr
+  | [ |- fbody_trivial _ = _ ] =>
+      unfold fbody_trivial;
+      _gnorm_itr
+  | [ |- cput _ _ = _ ] =>
+      unfold cput;
+      _gnorm_itr
+  | [ |- cgetU _ = _ ] =>
+      unfold cgetU;
+      _gnorm_itr
+  | [ |- cgetN _ = _ ] =>
+      unfold cgetN;
+      _gnorm_itr
+  | [ |- cfunU _ _ = _ ] =>
+      unfold cfunU;
+      _gnorm_itr
+  | [ |- cfunN _ _ = _ ] =>
+      unfold cfunN;
+      _gnorm_itr
+  | [ |- ccallU _ _ = _ ] =>
+      unfold ccallU;
+      _gnorm_itr
+  | [ |- ccallN _ _ = _ ] =>
+      unfold ccallN;
+      _gnorm_itr
+  | [ |- triggerUB = _ ] =>
+      unfold triggerUB;
+      _gnorm_itr
+  | [ |- triggerNB = _ ] =>
+      unfold triggerNB;
+      _gnorm_itr
+  | [ |- ?itr = _ ] =>
+      reflexivity
+end.
+Ltac gnorm_itr :=
+etransitivity;
+[ _gnorm_itr
+| s;
+  lazymatch goal with
+  | [ |- Ret _ = _ ] =>
+      reflexivity
+  | [ |- Tau _ = _ ] =>
+      reflexivity
+  | [ |- vis _ _ = _ ] =>
+      eapply vis_trigger
+  | [ |- _ = _ ] =>
+      reflexivity
+  end
+].
+
+Ltac norm_l :=
+  replace_l; [s; gnorm_itr|].
+Ltac norm_r :=
+  replace_r; [s; gnorm_itr|].
+
+Ltac iter_l :=
+  replace_l; [rewrite unfold_iterV /itreeV_itree //|]; norm_l.
+Ltac iter_r :=
+  replace_r; [rewrite unfold_iterV /itreeV_itree //|]; norm_r.
+
+Ltac step_r :=
+  norm_r; guclo gsim_indC_spec; econs; instantiate (1:=smj_top).
+Ltac step_l :=
+  norm_l; guclo gsim_indC_spec; econs; instantiate (1:=smj_top).
+
+Ltac replace_tp_r :=
+  match goal with
+  | |- gpaco7 _ _ _ _ _ _ _ _ _ _ (LModTr.interp_stateE _ (iterV _ ?tp) _) =>
+      pattern tp;
+      match goal with
+      | |- ?f ?tp =>
+          eapply (eq_ind_r f); cycle 1
+      end
+  end.
+Ltac replace_tp_l :=
+  match goal with
+  | |- gpaco7 _ _ _ _ _ _ _ _ _ (LModTr.interp_stateE _ (iterV _ ?tp) _) _ =>
+      pattern tp;
+      match goal with
+      | |- ?f ?tp =>
+          eapply (eq_ind_r f); cycle 1
+      end
+  end.
 
 Notation "'⇓cris'" := (interpV (ModTr.handle_crisE)).
 Notation "'⇓sb(' i ',' m ',' s ')'" := (interpV (SB.handle_sandbox i m s)).
@@ -429,6 +428,15 @@ Notation "'⇓smod(' img ',' sp ')'" := (interpV (SModTr.handle img sp)).
 
 Section props.
   Context `{!crisG Γ Σ α β τ _S _I, !concG, !newschG}.
+
+  Lemma gsim_flag r g RR p_s p_t i_s i_t :
+    gpaco7 _gsim (cpn7 _gsim) r g (Any.t * Any.t)%type (Any.t * Any.t)%type RR smj_bot smj_bot
+      i_s i_t →
+    gpaco7 _gsim (cpn7 _gsim) r g (Any.t * Any.t)%type (Any.t * Any.t)%type RR p_s p_t
+      i_s i_t.
+  Proof.
+    intros ?; guclo flagC_spec; econs; try instantiate (1:=smj_bot); eauto using smj_le_bot.
+  Qed.
 
   Lemma gsim_tau_src r g RR p_s p_t st_s st_t prog_s prog_t tid_s tid_t tp_s tp_t
       img_c msk_c scp_c k (k2 : Any.t → _) :
@@ -1105,7 +1113,6 @@ Section props.
     }
   Qed.
 
-
   Lemma gsim_jobs_both r g RR p_s p_t st_s st_t prog_s prog_t tid_s tid_t tp_s tp_t
       img_c msk_c scp_c k_s k_t (k_s1 k_t1 : Any.t → itree _ Any.t) (res : Σ) job :
     tid_s < length tp_s →
@@ -1130,7 +1137,7 @@ Section props.
         tp_t)) (Any.pair st_t (res↑))).
   Proof.
     intros Hlen_s Hlen_t Hres Hk.
-    guclo flagC_spec; econs; try instantiate (1:=smj_bot); eauto using smj_le_bot.
+    apply gsim_flag.
     revert Hres; generalize job res. clear job res.
     gcofix CIH.
     intros job res Hres.
@@ -1148,7 +1155,7 @@ Section props.
       eapply gsim_tau_tgt; [rewrite list_lookup_insert //|rewrite list_insert_insert].
       { rewrite interpV_tau //. }
       zprogress.
-      guclo flagC_spec; econs; try instantiate (1:=smj_bot); eauto using smj_le_bot.
+      apply gsim_flag.
       gbase. eapply CIH; eauto using list_lookup_insert.
     }
     { (* agE *)
@@ -1166,7 +1173,7 @@ Section props.
           }
           exists r_s2; esplits; try by des.
           zprogress.
-          guclo flagC_spec; econs; try instantiate (1:=smj_bot); eauto using smj_le_bot.
+          apply gsim_flag.
           gbase. eapply CIH; eauto using list_lookup_insert.
           by des.
         }
@@ -1182,7 +1189,7 @@ Section props.
           }
           split; first done.
           zprogress.
-          guclo flagC_spec; econs; try instantiate (1:=smj_bot); eauto using smj_le_bot.
+          apply gsim_flag.
           gbase. eapply CIH; eauto using list_lookup_insert.
         }
         { rewrite /Helping.trans (bisim_is_eq (translate_vis _ _ _ _)). ired.
@@ -1197,7 +1204,7 @@ Section props.
           }
           exists r_t2; split; first done.
           zprogress.
-          guclo flagC_spec; econs; try instantiate (1:=smj_bot); eauto using smj_le_bot.
+          apply gsim_flag.
           gbase. eapply CIH; eauto using list_lookup_insert.
           by des.
         }
@@ -1212,7 +1219,7 @@ Section props.
             [rewrite list_lookup_insert //=|exists x; rewrite list_insert_insert].
           { instantiate (1:=k_s1). rewrite vis_bind interpV_vis; repeat f_equal; grind. }
           zprogress.
-          guclo flagC_spec; econs; try instantiate (1:=smj_bot); eauto using smj_le_bot.
+          apply gsim_flag.
           gbase. eapply CIH; eauto using list_lookup_insert.
         }
         { rewrite /Helping.trans (bisim_is_eq (translate_vis _ _ _ _)). ired.
@@ -1224,7 +1231,7 @@ Section props.
             [rewrite list_lookup_insert //=|exists x; rewrite list_insert_insert].
           { instantiate (1:=k_t1). rewrite vis_bind interpV_vis; repeat f_equal; grind. }
           split; first done. zprogress.
-          guclo flagC_spec; econs; try instantiate (1:=smj_bot); eauto using smj_le_bot.
+          apply gsim_flag.
           gbase. eapply CIH; eauto using list_lookup_insert.
         }
         { iter_l. rewrite list_lookup_insert //=.
@@ -1234,12 +1241,617 @@ Section props.
           intros ?? ->.
           step_l; step_r. norm_l; norm_r. rewrite ?list_insert_insert. ired.
           zprogress.
-          guclo flagC_spec; econs; try instantiate (1:=smj_bot); eauto using smj_le_bot.
+          apply gsim_flag.
           gbase. eapply CIH; eauto using list_lookup_insert.
         }
       }
     }
   Unshelve. exact smj_top.
   Qed.
-
 End props.
+
+Ltac unfold_trans :=
+  rewrite /ModTr.trans_ktree /SB.sandbox_body /SB.sandbox
+    /ModTr.trans /SModTr.trans_ktree /SModTr.trans /=.
+
+Section Helping.
+  Context `{!crisG Γ Σ α β τ _S _I, !concG, !newschG}.
+  (* sp, module name for the helping module *)
+  Context (sp : sp_type) (mn : string).
+  Context (Hyield : sp SchHdr.yield = None ∨ ∃ E, sp SchHdr.yield = Some (SchA.yield_spec E)).
+  Context `{jobID} (jobs : jobID → itree Helping.pureE unit).
+  Context (msk : string → bool). (* mask for the user module *)
+
+  Definition mod_on :=  (HelpingOn.t mn jobs sp)  ★ (CFilter.filter msk SchI.t).
+  Definition mod_off := (HelpingOff.t mn jobs sp) ★ (CFilter.filter msk SchI.t).
+
+  Lemma get_tid_run_neq : SchHdr.get_tid ≠ Helping.run mn.
+  Proof.
+    rewrite /SchHdr.get_tid /Helping.run; destruct (decide (String.length mn = 7)) as [Hlen|];
+      cycle 1.
+    { assert (Hlen : String.length "Sch.get_tid" = 11) by ss.
+      intros Heq; rewrite Heq string_length_app in Hlen; ss; lia.
+    }
+    rewrite -get_correct; intros Hfalse; specialize (Hfalse (3 + String.length mn)).
+    rewrite -(append_correct2 _ _) Hlen in Hfalse; ss.
+  Qed.
+
+  Lemma get_tid_help_neq : SchHdr.get_tid ≠ Helping.help mn.
+  Proof.
+    rewrite /SchHdr.get_tid /Helping.help; destruct (decide (String.length mn = 6)) as [Hlen|];
+      cycle 1.
+    { assert (Hlen : String.length "Sch.get_tid" = 11) by ss.
+      intros Heq; rewrite Heq string_length_app in Hlen; ss; lia.
+    }
+    rewrite -get_correct; intros Hfalse; specialize (Hfalse (3 + String.length mn)).
+    rewrite -(append_correct2 _ _) Hlen in Hfalse; ss.
+  Qed.
+
+  Lemma yield_run_neq : SchHdr.yield ≠ Helping.run mn.
+  Proof.
+    rewrite /SchHdr.yield /Helping.run; destruct (decide (String.length mn = 5)) as [Hlen|];
+      cycle 1.
+    { assert (Hlen : String.length "Sch.yield" = 9) by ss.
+      intros Heq; rewrite Heq string_length_app in Hlen; ss; lia.
+    }
+    rewrite -get_correct; intros Hfalse; specialize (Hfalse (3 + String.length mn)).
+    rewrite -(append_correct2 _ _) Hlen in Hfalse; ss.
+  Qed.
+
+  Lemma yield_help_neq : SchHdr.yield ≠ Helping.help mn.
+  Proof.
+    rewrite /SchHdr.yield /Helping.help; destruct (decide (String.length mn = 4)) as [Hlen|];
+      cycle 1.
+    { assert (Hlen : String.length "Sch.yield" = 9) by ss.
+      intros Heq; rewrite Heq string_length_app in Hlen; ss; lia.
+    }
+    rewrite -get_correct; intros Hfalse; specialize (Hfalse (0 + String.length mn)).
+    rewrite -(append_correct2 _ _) Hlen in Hfalse; ss.
+  Qed.
+
+  Lemma join_run_neq : SchHdr.join ≠ Helping.run mn.
+  Proof.
+    rewrite /SchHdr.join /Helping.run; destruct (decide (String.length mn = 4)) as [Hlen|];
+      cycle 1.
+    { assert (Hlen : String.length "Sch.join" = 8) by ss.
+      intros Heq; rewrite Heq string_length_app in Hlen; ss; lia.
+    }
+    rewrite -get_correct; intros Hfalse; specialize (Hfalse (1 + String.length mn)).
+    rewrite -(append_correct2 _ _) Hlen in Hfalse; ss.
+  Qed.
+
+  Lemma join_help_neq : SchHdr.join ≠ Helping.help mn.
+  Proof.
+    rewrite /SchHdr.join /Helping.help; destruct (decide (String.length mn = 3)) as [Hlen|];
+      cycle 1.
+    { assert (Hlen : String.length "Sch.join" = 8) by ss.
+      intros Heq; rewrite Heq string_length_app in Hlen; ss; lia.
+    }
+    rewrite -get_correct; intros Hfalse; specialize (Hfalse (1 + String.length mn)).
+    rewrite -(append_correct2 _ _) Hlen in Hfalse; ss.
+  Qed.
+
+  Notation prog_s ctx rs := (LMod.prog
+    (Mod.to_lmod
+      ((SMod.to_mod sp (HelpingOff.Mod mn jobs)
+      ★ CFilter.filter msk (SMod.to_mod sp_none SchI.smod)) ★ ctx) rs)).
+  Notation prog_t ctx rs := (LMod.prog
+    (Mod.to_lmod
+      ((SMod.to_mod sp (HelpingOn.Mod mn jobs sp)
+      ★ CFilter.filter msk (SMod.to_mod sp_none SchI.smod)) ★ ctx) rs)).
+
+  Definition run_s : Any.t → itree lmodE Any.t := λ x,
+    ⇓cris (⇓sb(true, wmask_all, HelpingOff.scopes mn)
+      (tau;; ⇓smod(true, sp) (HelpingOff.run jobs x))).
+  Definition run_t : Any.t → itree lmodE Any.t := λ x,
+    ⇓cris (⇓sb(true, wmask_all, HelpingOn.scopes mn)
+      (tau;; ⇓smod(true, sp) (HelpingOn.run mn jobs x))).
+
+  Definition help_s : Any.t → itree lmodE Any.t := λ x,
+    ⇓cris (⇓sb(true, wmask_all, HelpingOff.scopes mn)
+      (tau;; ⇓smod(true, sp) (HelpingOff.help x))).
+  Definition help_t : Any.t → itree lmodE Any.t := λ x,
+    ⇓cris (⇓sb(true, wmask_all, HelpingOn.scopes mn)
+      (tau;; ⇓smod(true, sp) (HelpingOn.help mn jobs sp x))).
+
+  Definition yield : Any.t → itree lmodE Any.t := λ x,
+    ⇓cris (⇓sb(false, wmask_and msk wmask_all, SchI.scopes)
+      (tau;; ⇓smod(false, sp_none) (cfunU SchI.yield x))).
+  Definition inner_spawn : Any.t → itree lmodE Any.t := λ x,
+    ⇓cris (⇓sb(false, wmask_and msk wmask_all, SchI.scopes)
+      (tau;; ⇓smod(false, sp_none) (cfunU SchI.inner_spawn x))).
+  Definition spawn : Any.t → itree lmodE Any.t := λ x,
+    ⇓cris (⇓sb(false, wmask_and msk wmask_all, SchI.scopes)
+      (tau;; ⇓smod(false, sp_none) (cfunU SchI.spawn x))).
+  Definition join : Any.t → itree lmodE Any.t := λ x,
+    ⇓cris (⇓sb(false, wmask_and msk wmask_all, SchI.scopes)
+      (tau;; ⇓smod(false, sp_none) (cfunU SchI.join x))).
+  Definition get_tid : Any.t → itree lmodE Any.t := λ x,
+    ⇓cris (⇓sb(false, wmask_and msk wmask_all, SchI.scopes)
+      (tau;; ⇓smod(false, sp_none) (cfunU SchI.get_tid x))).
+
+  Lemma no_help_prog fn ctx rs :
+    fn ≠ Helping.run mn →
+    fn ≠ Helping.help mn →
+    prog_s ctx rs fn = prog_t ctx rs fn.
+  Proof.
+    intros ??.
+    rewrite /LMod.prog /=;
+    repeat (
+      match goal with
+      | |- context [dec ?a ?b] => destruct (dec a b); ss; clarify
+      end); esplits; eauto.
+  Qed.
+
+  Lemma prog_fn fn ctx rs :
+    Mod.wf ((HelpingOn.t mn jobs sp ★ CFilter.filter msk SchI.t) ★ ctx) →
+    (fn = Helping.run mn ∧ prog_s ctx rs fn = Some run_s ∧ prog_t ctx rs fn = Some run_t) ∨
+    (fn = Helping.help mn ∧ prog_s ctx rs fn = Some help_s ∧ prog_t ctx rs fn = Some help_t) ∨
+    prog_s ctx rs fn = prog_t ctx rs fn ∧
+    ((fn = SchHdr.yield ∧ prog_s ctx rs fn = Some yield) ∨
+     (fn = SchHdr.join ∧ prog_s ctx rs fn = Some join) ∨
+     (fn = SchHdr._spawn ∧ prog_s ctx rs fn = Some inner_spawn) ∨
+     (fn = SchHdr.spawn ∧ prog_s ctx rs fn = Some spawn) ∨
+     (fn = SchHdr.get_tid ∧ prog_s ctx rs fn = Some get_tid) ∨
+     (Some fn ∉ List.map fst (Mod.fnsems ((HelpingOn.t mn jobs sp) ★ (CFilter.filter msk SchI.t))) ∧
+     (prog_s ctx rs fn = None ∨
+     ∃ itr_ctx img1 msk1 scp1, (prog_s ctx rs fn =
+      Some (λ x, ⇓cris (⇓sb(img1, msk1, scp1) (itr_ctx x))) ∧
+      (scp1 ## (SchI.scopes ++ HelpingOff.scopes mn)))))).
+  Proof.
+    intros WF.
+    destruct (decide (fn = Helping.run mn)).
+    { subst; left.
+      rewrite /LMod.prog /=; destruct (dec _ _); last clarify; ss.
+    }
+    destruct (decide (fn = Helping.help mn)).
+    { subst; right; left.
+      rewrite /LMod.prog /=; destruct (dec _ _) as [e|e]; clarify; ss.
+      { rewrite /Helping.help /Helping.run in e; inv e. }
+      destruct (dec _ _); clarify; ss.
+    }
+    right; right. split; first apply no_help_prog; eauto.
+    destruct (decide (fn = SchHdr.yield)).
+    { left; subst; split; ss.
+      rewrite /LMod.prog /=; destruct (dec _ _) as [e|e]; ss; eauto; clarify; ss.
+      rewrite /LMod.prog /=; destruct (dec _ _) as [?|?]; ss; eauto; clarify; ss.
+    }
+    right.
+    destruct (decide (fn = SchHdr.join)).
+    { left; subst; split; ss.
+      rewrite /LMod.prog /=; destruct (dec _ _) as [?|?]; ss; eauto; clarify; ss.
+      rewrite /LMod.prog /=; destruct (dec _ _) as [?|?]; ss; eauto; clarify; ss.
+    }
+    right.
+    destruct (decide (fn = SchHdr._spawn)).
+    { left; subst; split; ss.
+      rewrite /LMod.prog /=; destruct (dec _ _) as [?|?]; ss; eauto; clarify; ss.
+      rewrite /LMod.prog /=; destruct (dec _ _) as [?|?]; ss; eauto; clarify; ss.
+    }
+    right.
+    destruct (decide (fn = SchHdr.spawn)).
+    { left; subst; split; ss.
+      rewrite /LMod.prog /=; destruct (dec _ _) as [?|?]; ss; eauto; clarify; ss.
+      rewrite /LMod.prog /=; destruct (dec _ _) as [?|?]; ss; eauto; clarify; ss.
+    }
+    right.
+    destruct (decide (fn = SchHdr.get_tid)).
+    { left; subst; split; ss.
+      rewrite /LMod.prog /=; destruct (dec _ _) as [?|?]; ss; eauto; clarify; ss.
+      rewrite /LMod.prog /=; destruct (dec _ _) as [e|e]; ss; eauto; clarify; ss.
+    }
+    right.
+    rewrite /LMod.prog /=.
+    repeat (destruct (dec _ _) as [e|e]; ss; [inv e; by clarify|clear e]).
+    rewrite /HelpingOn.t /SchI.t; unseal CRIS; ss.
+    split.
+    { set_solver. }
+    rewrite alist_find_map_snd.
+    destruct (alist_find (Some fn) (Mod.fnsems ctx)) as [[[[img1 msk1] scp1] itr_fn]|] eqn : Hfn.
+    { right; ss. esplits; eauto; ss.
+      hexploit (Mod.well_scoped_fns ctx (Some fn)); ss.
+      rewrite /fnsems_scopes Hfn /=; intros Hin.
+      apply elem_of_disjoint; intros x Hinctx%elem_of_list_In%Hin%elem_of_list_In Hinsch.
+      hexploit (Mod.wf_scopes); eauto; rewrite /Mod.scopes /=.
+      intros Hnodup; eapply (NoDup_app_disjoint _ _ Hnodup x); eauto.
+      { eapply elem_of_list_In. rewrite /Mod.scopes /SchI.t /HelpingOn.t; unseal CRIS; ss.
+        revert Hinsch; rewrite /HelpingOn.scopes /SchI.scopes; ss.
+        set_solver.
+      }
+      { eapply elem_of_list_In, Hinctx; eauto. }
+    }
+    left; ss.
+  Qed.
+
+  Lemma prog_fn_ctx fn ctx rs :
+    Mod.wf ((HelpingOn.t mn jobs sp ★ CFilter.filter msk SchI.t) ★ ctx) →
+    (Some fn ∉ List.map fst (Mod.fnsems ((HelpingOn.t mn jobs sp) ★ (CFilter.filter msk SchI.t)))) →
+    (prog_s ctx rs fn = None ∨
+     ∃ itr_ctx img1 msk1 scp1,
+      prog_t ctx rs fn = prog_s ctx rs fn ∧
+      prog_s ctx rs fn =
+        Some (λ x, ⇓cris (⇓sb(img1, msk1, scp1) (itr_ctx x))) ∧
+        (scp1 ## (SchI.scopes ++ HelpingOff.scopes mn))).
+  Proof.
+    intros ? NIN; hexploit (prog_fn fn ctx rs); eauto; intros CASE.
+    revert NIN; rewrite /HelpingOn.t /SchI.t; unseal CRIS; ss.
+    destruct CASE as [[-> ?]|CASE]; first set_solver.
+    destruct CASE as [[-> ?]|[-> CASE]]; first set_solver.
+    destruct CASE as [[-> ?]|CASE]; first set_solver.
+    destruct CASE as [[-> ?]|CASE]; first set_solver.
+    destruct CASE as [[-> ?]|CASE]; first set_solver.
+    destruct CASE as [[-> ?]|CASE]; first set_solver.
+    destruct CASE as [[-> ?]|CASE]; first set_solver.
+    i; des; eauto. right; esplits; eauto.
+  Qed.
+
+  Lemma prog_s_prog_t fn ctx rs itr :
+    Mod.wf ((HelpingOn.t mn jobs sp ★ CFilter.filter msk SchI.t) ★ ctx) →
+    prog_s ctx rs fn = Some itr →
+    (prog_t ctx rs fn = Some itr ∨
+     (fn = Helping.run mn ∧ itr = run_s ∧ prog_t ctx rs fn = Some run_t) ∨
+     (fn = Helping.help mn ∧ itr = help_s ∧ prog_t ctx rs fn = Some help_t)).
+  Proof.
+    intros ? Hs; hexploit (prog_fn fn ctx rs); eauto.
+    i; des; clarify; eauto; left; rewrite -H3 //.
+  Qed.
+
+  Lemma yield_unfold :
+    @Sch.yield crisE _ _ =
+    tau;; b <- trigger (Choose (option bool));;
+    match b with
+    | None => Ret tt
+    | Some false => Sch.yield
+    | Some true => trigger (Call SchHdr.yield tt↑);;; Sch.yield
+    end.
+  Proof.
+    rewrite {1}/Sch.yield; unseal SCH; rewrite unfold_iterC.
+    repeat f_equal. ired. repeat f_equal. extensionalities b. destruct b as [[|]|]; ss.
+    { ired. f_equal. extensionalities x. rewrite /Sch.yield; unseal SCH; ss. }
+    { ired. rewrite /Sch.yield; unseal SCH; ss. }
+    { ired. done. }
+  Qed.
+
+  Definition reqmap_rel
+      (tl : list (itree lmodE Any.t * itree lmodE Any.t * option (nat * (bool * jobID))))
+      (reqmap : gmap nat (bool * jobID)) : Prop :=
+    NoDup (omap id tl.*2).*1 ∧
+    (∀ stid rid jid b,
+      (tl.*2 !! stid = Some (Some (rid, (b, jid))) → reqmap !! rid = Some (b, jid))) ∧
+    (∀ rid jid, reqmap !! rid = Some (true, jid) →
+      ∃ stid, tl.*2 !! stid = Some (Some (rid, (true, jid)))).
+
+  Lemma reqmap_rel_id stid es0 es1 r tl reqmap :
+    tl !! stid = Some (es0, r) →
+    reqmap_rel tl reqmap →
+    reqmap_rel (<[stid:=(es1, r)]> tl) reqmap.
+  Proof.
+    intros [tl1 [tl2 [-> Hlen]]]%elem_of_list_split_length.
+    rewrite -(Nat.add_0_r stid); subst stid; rewrite /reqmap_rel insert_app_r ?fmap_app; cbn.
+    rewrite ?omap_app ?fmap_app; cbn; destruct r; eauto.
+  Qed.
+
+  Lemma reqmap_rel_Some tl reqmap stid rid b jid es :
+    tl !! stid = Some (es, Some (rid, (b, jid))) →
+    reqmap_rel tl reqmap →
+    reqmap !! rid = Some (b, jid).
+  Proof.
+    rewrite /reqmap_rel; intros Hin [Hnodup [Hrel1 Hrel2]].
+    apply (Hrel1 stid rid jid b). rewrite list_lookup_fmap Hin; eauto.
+  Qed.
+
+  Lemma reqmap_rel_Some_2 tl reqmap (i_s i_t : itree lmodE Any.t) rid jid :
+    reqmap_rel tl reqmap →
+    reqmap !! rid = Some (true, jid) →
+    ∃ stid i_s i_t, tl !! stid = Some (i_s, i_t, Some (rid, (true, jid))).
+  Proof.
+    rewrite /reqmap_rel; intros [? [? Hsome]] [stid Hstid]%Hsome; exists stid.
+    apply list_lookup_fmap_inv in Hstid as [[[? ?] [[? [? ?]]|]] [? ?]]; ss.
+    clarify; esplits; eauto.
+  Qed.
+
+  Lemma reqmap_rel_delete_true tl stid rid jid es0 es1 reqmap :
+    tl !! stid = Some (es0, Some (rid, (true, jid))) →
+    reqmap_rel tl reqmap →
+    reqmap_rel (<[stid := (es1, None)]> tl) (<[rid := (false, jid)]> reqmap).
+  Proof.
+    intros Hin [Hnodup [Hrel1 Hrel2]]; eapply lookup_lt_Some in Hin as Hlen; split.
+    { revert Hin; intros [tl1 [tl2 [-> ?]]]%elem_of_list_split_length.
+      rewrite -(Nat.add_0_r stid); subst stid; rewrite /reqmap_rel insert_app_r ?fmap_app; cbn.
+      rewrite ?omap_app ?fmap_app; cbn.
+      revert Hnodup; rewrite cons_app Permutation_app_swap_app; cbn.
+      rewrite ?fmap_app ?omap_app ?fmap_app. apply NoDup_cons.
+    }
+    split.
+    { intros stid1 rid1 jid1 b1 Hstid1.
+      rewrite list_lookup_fmap in Hstid1.
+      destruct (decide (stid = stid1)); subst.
+      { rewrite list_lookup_insert // in Hstid1. }
+      rewrite list_lookup_insert_ne // in Hstid1.
+      rewrite lookup_insert_ne; [eapply Hrel1; rewrite list_lookup_fmap; eauto|].
+      ii; clarify.
+      revert Hin; intros [tl1 [tl2 [-> ->]]]%elem_of_list_split_length.
+      revert Hnodup; rewrite cons_app Permutation_app_swap_app; cbn.
+      intros Hnodup; apply NoDup_cons in Hnodup; apply Hnodup.
+      apply elem_of_list_fmap; exists (rid1, (b1, jid1)); split; ss.
+      apply elem_of_list_omap; exists (Some (rid1, (b1, jid1))); split; ss.
+      rewrite -list_lookup_fmap in Hstid1.
+      apply list_lookup_fmap_inv in Hstid1 as [[[? ?] ?] [? Hstid]]; ss; clarify.
+      apply lookup_app_Some in Hstid; des; ss.
+      { rewrite fmap_app; apply elem_of_app; left.
+        apply elem_of_list_fmap; esplits; [|apply elem_of_list_lookup]; eauto; ss.
+      }
+      rewrite lookup_cons in Hstid0; des_ifs; first lia.
+      rewrite fmap_app; apply elem_of_app; right.
+      apply elem_of_list_fmap; esplits; [|apply elem_of_list_lookup]; eauto; ss.
+    }
+    intros rid1 jid1; destruct (decide (rid1 = rid)).
+    { subst; rewrite lookup_insert; i; clarify. }
+    rewrite lookup_insert_ne //; intros [stid1 Hstid1]%Hrel2.
+    exists stid1; rewrite list_fmap_insert /= list_lookup_insert_ne //.
+    ii; clarify.
+    rewrite list_lookup_fmap Hin /= in Hstid1; clarify.
+  Qed.
+
+  Lemma reqmap_rel_delete_true_2 tl stid rid jid es0 es1 reqmap :
+    tl !! stid = Some (es0, Some (rid, (true, jid))) →
+    reqmap_rel tl reqmap →
+    reqmap_rel (<[stid := (es1, Some (rid, (false, jid)))]> tl) (<[rid := (false, jid)]> reqmap).
+  Proof.
+    intros Hin [Hnodup [Hrel1 Hrel2]]; eapply lookup_lt_Some in Hin as Hlen; split.
+    { revert Hin; intros [tl1 [tl2 [-> ?]]]%elem_of_list_split_length.
+      rewrite -(Nat.add_0_r stid); subst stid; rewrite /reqmap_rel insert_app_r ?fmap_app; cbn.
+      revert Hnodup; rewrite ?fmap_app ?omap_app ?fmap_app //; cbn.
+    }
+    split.
+    { intros stid1 rid1 jid1 b1 Hstid1.
+      rewrite list_lookup_fmap in Hstid1.
+      destruct (decide (stid = stid1)); subst.
+      { rewrite list_lookup_insert //= in Hstid1; clarify. rewrite lookup_insert //. }
+      rewrite list_lookup_insert_ne // in Hstid1.
+      rewrite lookup_insert_ne; [eapply Hrel1; rewrite list_lookup_fmap; eauto|].
+      ii; clarify.
+      revert Hin; intros [tl1 [tl2 [-> ->]]]%elem_of_list_split_length.
+      revert Hnodup; rewrite cons_app Permutation_app_swap_app; cbn.
+      intros Hnodup; apply NoDup_cons in Hnodup; apply Hnodup.
+      apply elem_of_list_fmap; exists (rid1, (b1, jid1)); split; ss.
+      apply elem_of_list_omap; exists (Some (rid1, (b1, jid1))); split; ss.
+      rewrite -list_lookup_fmap in Hstid1.
+      apply list_lookup_fmap_inv in Hstid1 as [[[? ?] ?] [? Hstid]]; ss; clarify.
+      apply lookup_app_Some in Hstid; des; ss.
+      { rewrite fmap_app; apply elem_of_app; left.
+        apply elem_of_list_fmap; esplits; [|apply elem_of_list_lookup]; eauto; ss.
+      }
+      rewrite lookup_cons in Hstid0; des_ifs; first lia.
+      rewrite fmap_app; apply elem_of_app; right.
+      apply elem_of_list_fmap; esplits; [|apply elem_of_list_lookup]; eauto; ss.
+    }
+    intros rid1 jid1; destruct (decide (rid1 = rid)).
+    { subst; rewrite lookup_insert; i; clarify. }
+    rewrite lookup_insert_ne //; intros [stid1 Hstid1]%Hrel2.
+    exists stid1; rewrite list_fmap_insert /= list_lookup_insert_ne //.
+    ii; clarify.
+    rewrite list_lookup_fmap Hin /= in Hstid1; clarify.
+  Qed.
+
+  Lemma reqmap_rel_delete_false tl stid rid jid es0 es1 reqmap :
+    tl !! stid = Some (es0, Some (rid, (false, jid))) →
+    reqmap_rel tl reqmap →
+    reqmap_rel (<[stid := (es1, None)]> tl) (reqmap).
+  Proof.
+    intros Hin [Hnodup [Hrel1 Hrel2]].
+    split.
+    { revert Hin; intros [tl1 [tl2 [-> Hlen]]]%elem_of_list_split_length.
+      rewrite -(Nat.add_0_r stid); subst stid; rewrite /reqmap_rel insert_app_r ?fmap_app; cbn.
+      rewrite ?omap_app ?fmap_app; cbn.
+      revert Hnodup; rewrite cons_app Permutation_app_swap_app; cbn.
+      rewrite ?fmap_app ?omap_app fmap_app. apply NoDup_cons.
+    }
+    split.
+    { intros stid' ??? Hstid'; eapply (Hrel1 stid'); eauto.
+      rewrite list_fmap_insert /= in Hstid'.
+      apply lookup_lt_Some in Hstid' as Hlen'. rewrite length_insert in Hlen'.
+      destruct (decide (stid = stid')); subst.
+      { rewrite list_lookup_insert // in Hstid'; ss. }
+      rewrite list_lookup_insert_ne // in Hstid'.
+    }
+    intros ?? [stid' Hlookup]%Hrel2; exists stid'.
+    rewrite list_fmap_insert /= list_lookup_insert_ne ?Hlookup //.
+    ii; clarify.
+    rewrite list_lookup_fmap Hin //= in Hlookup.
+  Qed.
+
+  Lemma reqmap_rel_insert_false tl reqmap rid jid :
+    rid ∉ (dom reqmap) →
+    reqmap_rel tl reqmap →
+    reqmap_rel tl (<[rid:=(false, jid)]> reqmap).
+  Proof.
+    intros Hrid [? [Hrel1 Hrel2]]; split; first done.
+    split.
+    { intros ???? Hstid%Hrel1.
+      rewrite lookup_insert_ne //.
+      ii; clarify; apply elem_of_dom_2 in Hstid; eauto.
+    }
+    intros rid1.
+    destruct (decide (rid = rid1)); subst; [rewrite lookup_insert|rewrite lookup_insert_ne]; eauto.
+    ii; clarify.
+  Qed.
+
+  Lemma reqmap_rel_insert_true tl reqmap stid es0 es1 rid jid :
+    rid ∉ (dom reqmap) →
+    tl !! stid = Some (es0, None) →
+    reqmap_rel tl reqmap →
+    reqmap_rel (<[stid:=(es1, Some (rid, (true, jid)))]> tl) (<[rid:=(true, jid)]> reqmap).
+  Proof.
+    intros Hrid Hin [Hnodup [Hrel1 Hrel2]]; eapply lookup_lt_Some in Hin as Hlen; split.
+    { rewrite insert_take_drop //.
+      rewrite ?fmap_app ?omap_app ?fmap_app; cbn.
+      rewrite cons_app Permutation_app_swap_app.
+      eapply take_drop_middle in Hin as Hmid; rewrite -Hmid in Hnodup; clear Hmid.
+      revert Hnodup; rewrite ?fmap_app ?omap_app fmap_app; cbn.
+      intros ?; apply NoDup_cons; split; eauto.
+      rewrite -fmap_app -omap_app -fmap_app.
+      intros [[? [? ?]] [? Hrid2]]%elem_of_list_fmap; ss; clarify.
+      apply elem_of_list_omap in Hrid2 as [[[? [? ?]] |] [Hrid2 ?]]; ss; clarify.
+      apply elem_of_list_fmap in Hrid2 as [[? [[? [? ?]] |]] [? Hrid2]]; ss; clarify.
+      apply Hrid, elem_of_dom.
+      assert (Hlem : (p, Some (n0, (b0, j0))) ∈ tl).
+      { eapply take_drop_middle in Hin as Hmid; rewrite -Hmid; clear Hmid. set_solver. }
+      apply elem_of_list_lookup in Hlem as [i Hlem].
+      hexploit (Hrel1 i); cycle 1.
+      { intros ->; ss. }
+      rewrite list_lookup_fmap Hlem //.
+    }
+    split.
+    { intros stid1 ? ? ?; destruct (decide (stid1 = stid)); subst.
+      { rewrite list_lookup_fmap list_lookup_insert /=; i; clarify; rewrite lookup_insert //. }
+      rewrite list_fmap_insert list_lookup_insert_ne //; intros Hcont%Hrel1.
+      rewrite lookup_insert_ne //.
+      ii; clarify.
+      apply Hrid, elem_of_dom; eauto.
+    }
+    intros rid1.
+    destruct (decide (rid = rid1)); subst; [rewrite lookup_insert|rewrite lookup_insert_ne]; eauto.
+    { ii; clarify. exists stid; rewrite list_fmap_insert list_lookup_insert // length_fmap //. }
+    intros ? [??]%Hrel2; exists x; rewrite list_fmap_insert list_lookup_insert_ne //.
+    ii; clarify.
+    rewrite list_lookup_fmap Hin /= in H2; clarify.
+  Qed.
+
+  Lemma reqmap_rel_append tl reqmap es :
+    reqmap_rel tl reqmap →
+    reqmap_rel (tl ++ [(es, None)]) reqmap.
+  Proof.
+    rewrite /reqmap_rel ?fmap_app ?omap_app ?fmap_app app_nil_r; cbn.
+    intros [? [Hrel1 Hrel2]]; split; first done.
+    split.
+    { intros ????; rewrite lookup_app_Some; intros [?%Hrel1|[??%list_lookup_singleton_Some]]; eauto.
+      des; clarify.
+    }
+    { intros ?? [stid Hstid]%Hrel2; apply lookup_lt_Some in Hstid as Hlen.
+      exists stid; rewrite lookup_app_l //.
+    }
+  Qed.
+
+  Definition inner_spawn_pend (arg : Any.t) ktr : itree lmodE Any.t :=
+    tau;;
+    x <- ⇓cris (⇓sb(false, wmask_and msk wmask_all, SchI.scopes)
+      (⇓smod(false, sp_none) (
+        'arg : SAny.t <- (arg↓)?;;
+        'x1 : thpool <- (cgetU SchI.v_ths);;
+        'x2 : nat <- (cgetU SchI.v_tid);;
+        r <-
+          (match x1 !! x2 with
+          | Some (stid, _) =>
+              cput SchI.v_ths (<[x2 := (stid, Some arg)]> x1);;;
+              Sch.terminate
+          | None => triggerUB
+          end);;
+        Ret (r↑))));;
+    ktr x.
+
+  Definition join_pend (arg : Any.t) stid ktr : itree lmodE Any.t :=
+    tau;;
+    x <- ⇓cris (⇓sb(false, wmask_and msk wmask_all, SchI.scopes)
+      (⇓smod(false, sp_none) (
+        'arg : () <- (arg↓)?;;
+        x_3 <- iterC (λ _ : (),
+          'x_1 : thpool <- cgetU SchI.v_ths;;
+          match x_1 !! stid with
+          | Some (_, Some rv) => Ret (inr (Some rv))
+          | Some (_, None) =>
+              '() : _ <- ccallU SchHdr.yield tt;; Ret (inl ())
+          | None => Ret (inr None)
+          end
+        ) ();;
+        Ret (x_3↑))));;
+    ktr x.
+
+  Definition helpee_pend_s
+      (j : jobID) k
+      (fspo : option fspec) (x_fsp : fspec_option_meta fspo)
+      : itree lmodE Any.t :=
+    tau;;
+    r <- ⇓cris (⇓sb(true, wmask_all, HelpingOff.scopes mn) (
+      HoareCall_epilogue fspo x_fsp ()↑;;;
+      ⇓smod(true, sp) (𝒴;;; Helping.trans (jobs j);;; 𝒴;;; Ret ()↑)
+    ));;
+     (k r).
+
+  Definition helpee_pend_t
+      (tid_stid_cur : nat) (j : jobID) k
+      (fspo : option fspec) (x_fsp : fspec_option_meta fspo)
+      : itree lmodE Any.t :=
+    tau;;
+    r <- ⇓cris (⇓sb(true, wmask_all, HelpingOff.scopes mn) (
+      HoareCall_epilogue fspo x_fsp ()↑;;;
+      ⇓smod(true, sp) (𝒴;;; HelpingOn.try_run mn jobs tid_stid_cur;;; 𝒴;;; Ret (()↑))
+    ));; (k r).
+
+  Inductive help_rel : itree lmodE Any.t → itree lmodE Any.t → option (nat * (bool * jobID)) → Prop :=
+  | help_rel_ret ret : help_rel (Ret ret) (Ret ret) None
+  | help_rel_eq itr_s itr_t (k_s k_t : Any.t → _) itr img msk scp :
+      itr_t = ModTr.trans (SB.sandbox img msk scp itr) >>= k_t →
+      itr_s = ModTr.trans (SB.sandbox img msk scp itr) >>= k_s →
+      scp ## (SchI.scopes ++ HelpingOff.scopes mn) →
+      (∀ ret, itr ≠ Ret ret) →
+      (∀ ret, help_rel (k_s ret) (k_t ret) None) →
+      help_rel itr_s itr_t None
+  | help_rel_loop itr_s itr_t ktr_t ktr_s x :
+      itr_t = (tau;;
+        x_ <- ⇓cris(⇓sb(true, wmask_all, HelpingOn.scopes mn)
+          (x_2 <- HoareCall_epilogue (sp SchHdr.yield) x (()↑);;
+          ⇓smod(true, sp) (Ret x_2;;; 𝒴;;; Ret (()↑))));;
+        ktr_t x_) →
+      itr_s = (tau;;
+        x_ <- ⇓cris(⇓sb(true, wmask_all, HelpingOn.scopes mn)
+          (x_2 <- HoareCall_epilogue (sp SchHdr.yield) x (()↑);;
+          ⇓smod(true, sp) (Ret x_2;;; 𝒴;;; Ret (()↑))));;
+        ktr_s x_) →
+      (∀ ret, help_rel (ktr_s ret) (ktr_t ret) None) →
+      help_rel itr_s itr_t None
+  | help_rel_helpee_done tid jid itr_s itr_t x k_s k_t :
+      itr_t = helpee_pend_t tid jid k_t (sp SchHdr.yield) x →
+      itr_s = (tau;;
+        x_ <- ⇓cris(⇓sb(true, wmask_all, HelpingOn.scopes mn)
+          (x_2 <- HoareCall_epilogue (sp SchHdr.yield) x (()↑);;
+          ⇓smod(true, sp) (Ret x_2;;; 𝒴;;; Ret (()↑))));;
+        k_s x_) →
+      (∀ ret, help_rel (k_s ret) (k_t ret) None) →
+      help_rel itr_s itr_t (Some (tid, (false, jid)))
+  | help_rel_helpee_pend tid jid itr_s itr_t k_s k_t x_fsp :
+      itr_s = helpee_pend_s jid k_s (sp SchHdr.yield) x_fsp →
+      itr_t = helpee_pend_t tid jid k_t (sp SchHdr.yield) x_fsp →
+      (∀ ret, help_rel (k_s ret) (k_t ret) None) →
+      help_rel itr_s itr_t (Some (tid, (true, jid)))
+  | help_rel_call itr_s itr_t ktr_t ktr_s ktr_t1 ktr_s1 ctx rs fn arg :
+      Some fn ∈ List.map fst (Mod.fnsems ((HelpingOn.t mn jobs sp) ★ (CFilter.filter msk SchI.t))) →
+      Mod.wf ((HelpingOn.t mn jobs sp ★ CFilter.filter msk SchI.t) ★ ctx) →
+      prog_t ctx rs fn = Some ktr_t →
+      prog_s ctx rs fn = Some ktr_s →
+      itr_t = ktr_t arg >>= ktr_t1 →
+      itr_s = ktr_s arg >>= ktr_s1 →
+      (∀ ret, help_rel (ktr_s1 ret) (ktr_t1 ret) None) →
+      help_rel itr_s itr_t None
+  | help_rel_inner_spawn itr_s itr_t (arg : Any.t) ktr_s ktr_t :
+      itr_t = inner_spawn_pend arg ktr_t →
+      itr_s = inner_spawn_pend arg ktr_s →
+      (∀ ret, help_rel (ktr_s ret) (ktr_t ret) None) →
+      help_rel itr_s itr_t None
+  | help_rel_join itr_s itr_t (arg : Any.t) ktr_s ktr_t tid :
+      itr_t = join_pend arg tid ktr_t →
+      itr_s = join_pend arg tid ktr_s →
+      (∀ ret, help_rel (ktr_s ret) (ktr_t ret) None) →
+      help_rel itr_s itr_t None
+  | help_rel_terminate itr_s itr_t ktr_s ktr_t :
+      itr_s =
+        (x <- ⇓cris (⇓sb( false, wmask_and msk wmask_all, SchI.scopes)
+          (⇓smod( false, sp_none) (x_ <- Sch.terminate;; Ret x_↑)));;
+        ktr_s x) →
+      itr_t =
+        (x <- ⇓cris (⇓sb( false, wmask_and msk wmask_all, SchI.scopes)
+          (⇓smod( false, sp_none) (x_ <- Sch.terminate;; Ret x_↑)));;
+        ktr_t x) →
+      (∀ ret, help_rel (ktr_s ret) (ktr_t ret) None) →
+      help_rel itr_s itr_t None.
+End Helping.
