helping/HelpingOnOffproof.v
@@ -4,18 +4,22 @@ Require Import GSim GSimFacts GSimTactics.
 Require Import SchHeader SchI SchA.
 From CRIS.helping Require Import Header HelpingOn HelpingOff HelpingAux.
 
+Ltac unfold_trans :=
+  rewrite /ModTr.trans_ktree /SB.sandbox_body /SB.sandbox
+    /ModTr.trans /SModTr.trans_ktree /SModTr.trans /=.
+
 Section Helping.
   Context `{!crisG Γ Σ α β τ _S _I, !concG, !newschG}.
   (* sp, module name for the helping module *)
   Context (sp : sp_type) (mn : string).
-  Context (Hyield : sp SchHdr.yield = None ∨ ∃ E, sp SchHdr.yield = Some (SchA.yield_spec E)).
+  (* Context (Hyield : sp SchHdr.yield = None ∨ ∃ E, sp SchHdr.yield = Some (SchA.yield_spec E)). *)
   Context `{jobID} (jobs : jobID → itree Helping.pureE unit).
   Context (msk : string → bool). (* mask for the user module *)
 
-  Local Definition mod_on :=  (HelpingOn.t mn jobs sp)  ★ (CFilter.filter msk SchI.t).
-  Local Definition mod_off := (HelpingOff.t mn jobs sp) ★ (CFilter.filter msk SchI.t).
+  Definition mod_on :=  (HelpingOn.t mn jobs sp)  ★ (CFilter.filter msk SchI.t).
+  Definition mod_off := (HelpingOff.t mn jobs sp) ★ (CFilter.filter msk SchI.t).
 
-  Local Lemma get_tid_run_neq : SchHdr.get_tid ≠ Helping.run mn.
+  Lemma get_tid_run_neq : SchHdr.get_tid ≠ Helping.run mn.
   Proof.
     rewrite /SchHdr.get_tid /Helping.run; destruct (decide (String.length mn = 7)) as [Hlen|];
       cycle 1.
@@ -26,7 +30,7 @@ Section Helping.
     rewrite -(append_correct2 _ _) Hlen in Hfalse; ss.
   Qed.
 
-  Local Lemma get_tid_help_neq : SchHdr.get_tid ≠ Helping.help mn.
+  Lemma get_tid_help_neq : SchHdr.get_tid ≠ Helping.help mn.
   Proof.
     rewrite /SchHdr.get_tid /Helping.help; destruct (decide (String.length mn = 6)) as [Hlen|];
       cycle 1.
@@ -37,7 +41,7 @@ Section Helping.
     rewrite -(append_correct2 _ _) Hlen in Hfalse; ss.
   Qed.
 
-  Local Lemma yield_run_neq : SchHdr.yield ≠ Helping.run mn.
+  Lemma yield_run_neq : SchHdr.yield ≠ Helping.run mn.
   Proof.
     rewrite /SchHdr.yield /Helping.run; destruct (decide (String.length mn = 5)) as [Hlen|];
       cycle 1.
@@ -48,7 +52,7 @@ Section Helping.
     rewrite -(append_correct2 _ _) Hlen in Hfalse; ss.
   Qed.
 
-  Local Lemma yield_help_neq : SchHdr.yield ≠ Helping.help mn.
+  Lemma yield_help_neq : SchHdr.yield ≠ Helping.help mn.
   Proof.
     rewrite /SchHdr.yield /Helping.help; destruct (decide (String.length mn = 4)) as [Hlen|];
       cycle 1.
@@ -59,7 +63,7 @@ Section Helping.
     rewrite -(append_correct2 _ _) Hlen in Hfalse; ss.
   Qed.
 
-  Local Lemma join_run_neq : SchHdr.join ≠ Helping.run mn.
+  Lemma join_run_neq : SchHdr.join ≠ Helping.run mn.
   Proof.
     rewrite /SchHdr.join /Helping.run; destruct (decide (String.length mn = 4)) as [Hlen|];
       cycle 1.
@@ -70,7 +74,7 @@ Section Helping.
     rewrite -(append_correct2 _ _) Hlen in Hfalse; ss.
   Qed.
 
-  Local Lemma join_help_neq : SchHdr.join ≠ Helping.help mn.
+  Lemma join_help_neq : SchHdr.join ≠ Helping.help mn.
   Proof.
     rewrite /SchHdr.join /Helping.help; destruct (decide (String.length mn = 3)) as [Hlen|];
       cycle 1.
@@ -90,37 +94,37 @@ Section Helping.
       ((SMod.to_mod sp (HelpingOn.Mod mn jobs sp)
       ★ CFilter.filter msk (SMod.to_mod sp_none SchI.smod)) ★ ctx) rs)).
 
-  Local Definition run_s : Any.t → itree lmodE Any.t := λ x,
+  Definition run_s : Any.t → itree lmodE Any.t := λ x,
     ⇓cris (⇓sb(true, wmask_all, HelpingOff.scopes mn)
       (tau;; ⇓smod(true, sp) (HelpingOff.run jobs x))).
-  Local Definition run_t : Any.t → itree lmodE Any.t := λ x,
+  Definition run_t : Any.t → itree lmodE Any.t := λ x,
     ⇓cris (⇓sb(true, wmask_all, HelpingOn.scopes mn)
       (tau;; ⇓smod(true, sp) (HelpingOn.run mn jobs x))).
 
-  Local Definition help_s : Any.t → itree lmodE Any.t := λ x,
+  Definition help_s : Any.t → itree lmodE Any.t := λ x,
     ⇓cris (⇓sb(true, wmask_all, HelpingOff.scopes mn)
       (tau;; ⇓smod(true, sp) (HelpingOff.help x))).
-  Local Definition help_t : Any.t → itree lmodE Any.t := λ x,
+  Definition help_t : Any.t → itree lmodE Any.t := λ x,
     ⇓cris (⇓sb(true, wmask_all, HelpingOn.scopes mn)
       (tau;; ⇓smod(true, sp) (HelpingOn.help mn jobs sp x))).
 
-  Local Definition yield : Any.t → itree lmodE Any.t := λ x,
+  Definition yield : Any.t → itree lmodE Any.t := λ x,
     ⇓cris (⇓sb(false, wmask_and msk wmask_all, SchI.scopes)
       (tau;; ⇓smod(false, sp_none) (cfunU SchI.yield x))).
-  Local Definition inner_spawn : Any.t → itree lmodE Any.t := λ x,
+  Definition inner_spawn : Any.t → itree lmodE Any.t := λ x,
     ⇓cris (⇓sb(false, wmask_and msk wmask_all, SchI.scopes)
       (tau;; ⇓smod(false, sp_none) (cfunU SchI.inner_spawn x))).
-  Local Definition spawn : Any.t → itree lmodE Any.t := λ x,
+  Definition spawn : Any.t → itree lmodE Any.t := λ x,
     ⇓cris (⇓sb(false, wmask_and msk wmask_all, SchI.scopes)
       (tau;; ⇓smod(false, sp_none) (cfunU SchI.spawn x))).
-  Local Definition join : Any.t → itree lmodE Any.t := λ x,
+  Definition join : Any.t → itree lmodE Any.t := λ x,
     ⇓cris (⇓sb(false, wmask_and msk wmask_all, SchI.scopes)
       (tau;; ⇓smod(false, sp_none) (cfunU SchI.join x))).
-  Local Definition get_tid : Any.t → itree lmodE Any.t := λ x,
+  Definition get_tid : Any.t → itree lmodE Any.t := λ x,
     ⇓cris (⇓sb(false, wmask_and msk wmask_all, SchI.scopes)
       (tau;; ⇓smod(false, sp_none) (cfunU SchI.get_tid x))).
 
-  Local Lemma no_help_prog fn ctx rs :
+  Lemma no_help_prog fn ctx rs :
     fn ≠ Helping.run mn →
     fn ≠ Helping.help mn →
     prog_s ctx rs fn = prog_t ctx rs fn.
@@ -133,7 +137,8 @@ Section Helping.
       end); esplits; eauto.
   Qed.
 
-  Local Lemma prog_fn fn ctx rs :
+  Lemma prog_fn fn ctx rs :
+    Mod.wf ((HelpingOn.t mn jobs sp ★ CFilter.filter msk SchI.t) ★ ctx) →
     (fn = Helping.run mn ∧ prog_s ctx rs fn = Some run_s ∧ prog_t ctx rs fn = Some run_t) ∨
     (fn = Helping.help mn ∧ prog_s ctx rs fn = Some help_s ∧ prog_t ctx rs fn = Some help_t) ∨
     prog_s ctx rs fn = prog_t ctx rs fn ∧
@@ -142,8 +147,13 @@ Section Helping.
      (fn = SchHdr._spawn ∧ prog_s ctx rs fn = Some inner_spawn) ∨
      (fn = SchHdr.spawn ∧ prog_s ctx rs fn = Some spawn) ∨
      (fn = SchHdr.get_tid ∧ prog_s ctx rs fn = Some get_tid) ∨
-     Some fn ∉ List.map fst (Mod.fnsems ((HelpingOn.t mn jobs sp) ★ (CFilter.filter msk SchI.t)))).
+     (Some fn ∉ List.map fst (Mod.fnsems ((HelpingOn.t mn jobs sp) ★ (CFilter.filter msk SchI.t))) ∧
+     (prog_s ctx rs fn = None ∨
+     ∃ itr_ctx img1 msk1 scp1, (prog_s ctx rs fn =
+      Some (λ x, ⇓cris (⇓sb(img1, msk1, scp1) (itr_ctx x))) ∧
+      (scp1 ## (SchI.scopes ++ HelpingOff.scopes mn)))))).
   Proof.
+    intros WF.
     destruct (decide (fn = Helping.run mn)).
     { subst; left.
       rewrite /LMod.prog /=; destruct (dec _ _); last clarify; ss.
@@ -184,16 +194,60 @@ Section Helping.
       rewrite /LMod.prog /=; destruct (dec _ _) as [?|?]; ss; eauto; clarify; ss.
       rewrite /LMod.prog /=; destruct (dec _ _) as [e|e]; ss; eauto; clarify; ss.
     }
-    right. rewrite /HelpingOn.t /SchI.t; unseal CRIS; ss; set_solver.
+    right.
+    rewrite /LMod.prog /=.
+    repeat (destruct (dec _ _) as [e|e]; ss; [inv e; by clarify|clear e]).
+    rewrite /HelpingOn.t /SchI.t; unseal CRIS; ss.
+    split.
+    { set_solver. }
+    rewrite alist_find_map_snd.
+    destruct (alist_find (Some fn) (Mod.fnsems ctx)) as [[[[img1 msk1] scp1] itr_fn]|] eqn : Hfn.
+    { right; ss. esplits; eauto; ss.
+      hexploit (Mod.well_scoped_fns ctx (Some fn)); ss.
+      rewrite /fnsems_scopes Hfn /=; intros Hin.
+      apply elem_of_disjoint; intros x Hinctx%elem_of_list_In%Hin%elem_of_list_In Hinsch.
+      hexploit (Mod.wf_scopes); eauto; rewrite /Mod.scopes /=.
+      intros Hnodup; eapply (NoDup_app_disjoint _ _ Hnodup x); eauto.
+      { eapply elem_of_list_In. rewrite /Mod.scopes /SchI.t /HelpingOn.t; unseal CRIS; ss.
+        revert Hinsch; rewrite /HelpingOn.scopes /SchI.scopes; ss.
+        set_solver.
+      }
+      { eapply elem_of_list_In, Hinctx; eauto. }
+    }
+    left; ss.
+  Qed.
+
+  Lemma prog_fn_ctx fn ctx rs :
+    Mod.wf ((HelpingOn.t mn jobs sp ★ CFilter.filter msk SchI.t) ★ ctx) →
+    (Some fn ∉ List.map fst (Mod.fnsems ((HelpingOn.t mn jobs sp) ★ (CFilter.filter msk SchI.t)))) →
+    (prog_s ctx rs fn = None ∨
+     ∃ itr_ctx img1 msk1 scp1,
+      prog_t ctx rs fn = prog_s ctx rs fn ∧
+      prog_s ctx rs fn =
+        Some (λ x, ⇓cris (⇓sb(img1, msk1, scp1) (itr_ctx x))) ∧
+        (scp1 ## (SchI.scopes ++ HelpingOff.scopes mn))).
+  Proof.
+    intros ? NIN; hexploit (prog_fn fn ctx rs); eauto; intros CASE.
+    revert NIN; rewrite /HelpingOn.t /SchI.t; unseal CRIS; ss.
+    destruct CASE as [[-> ?]|CASE]; first set_solver.
+    destruct CASE as [[-> ?]|[-> CASE]]; first set_solver.
+    destruct CASE as [[-> ?]|CASE]; first set_solver.
+    destruct CASE as [[-> ?]|CASE]; first set_solver.
+    destruct CASE as [[-> ?]|CASE]; first set_solver.
+    destruct CASE as [[-> ?]|CASE]; first set_solver.
+    destruct CASE as [[-> ?]|CASE]; first set_solver.
+    i; des; eauto. right; esplits; eauto.
   Qed.
 
   Lemma prog_s_prog_t fn ctx rs itr :
+    Mod.wf ((HelpingOn.t mn jobs sp ★ CFilter.filter msk SchI.t) ★ ctx) →
     prog_s ctx rs fn = Some itr →
     (prog_t ctx rs fn = Some itr ∨
      (fn = Helping.run mn ∧ itr = run_s ∧ prog_t ctx rs fn = Some run_t) ∨
      (fn = Helping.help mn ∧ itr = help_s ∧ prog_t ctx rs fn = Some help_t)).
   Proof.
-    intros Hs; hexploit (prog_fn fn ctx rs); i; des; clarify; eauto; try by (left; rewrite -H2 //).
+    intros ? Hs; hexploit (prog_fn fn ctx rs); eauto.
+    i; des; clarify; eauto; left; rewrite -H3 //.
   Qed.
 
   Lemma yield_unfold :
@@ -432,212 +486,43 @@ Section Helping.
       exists stid; rewrite lookup_app_l //.
     }
   Qed.
-  (* Definition reqlist
-      (tl : list (itree lmodE Any.t * itree lmodE Any.t * option (nat * (bool * jobID))))
-      : list (nat * (bool * jobID)) :=
-    omap id tl.*2. *)
 
-  (* Definition reqmap_tl tl : gmap nat (bool * jobID) := list_to_map (reqlist tl). *)
+  Definition inner_spawn_pend (arg : Any.t) ktr : itree lmodE Any.t :=
+    tau;;
+    x <- ⇓cris (⇓sb(false, wmask_and msk wmask_all, SchI.scopes)
+      (⇓smod(false, sp_none) (
+        'arg : SAny.t <- (arg↓)?;;
+        'x1 : thpool <- (cgetU SchI.v_ths);;
+        'x2 : nat <- (cgetU SchI.v_tid);;
+        r <-
+          (match x1 !! x2 with
+          | Some (stid, _) =>
+              cput SchI.v_ths (<[x2 := (stid, Some arg)]> x1);;;
+              Sch.terminate
+          | None => triggerUB
+          end);;
+        Ret (r↑))));;
+    ktr x.
 
-  (* Lemma reqlist_Some_None tl stid rid e0 e1 o0 o1 reqmap :
-    NoDup (reqlist tl).*1 →
-    tl !! stid = Some (e0, Some (rid, o0)) →
-    reqmap_tl tl ⊆ reqmap →
-    reqmap_tl (<[stid := (e1, None)]> tl) ⊆ <[rid := o1]> reqmap.
-  Proof.
-    intros Hnodup Hin; rewrite /reqmap_tl /reqlist.
-    eapply elem_of_list_split_length in Hin as [tl1 [tl2 [-> Hlen]]].
-    rewrite -(Nat.add_0_r stid); subst stid; rewrite insert_app_r /=.
-    rewrite ?fmap_app ?omap_app; cbn; intros Hsub.
-    eapply map_subseteq_spec; intros i x Hi.
-    destruct (decide (i = rid)).
-    { exfalso; subst.
-      revert Hnodup; rewrite /reqlist fmap_app omap_app; cbn.
-      rewrite cons_app Permutation_app_swap_app; cbn.
-      move => /NoDup_cons; intros [Hnin _]; apply Hnin.
-      apply elem_of_list_to_map_2 in Hi.
-      eapply elem_of_list_fmap; exists (rid, x); ss.
-    }
-    rewrite lookup_insert_ne //; eapply lookup_weaken; eauto.
-    etrans; last apply Hsub.
-    eapply map_subseteq_spec; intros a ? ?%elem_of_list_to_map_2%elem_of_app.
-    eapply elem_of_list_to_map_1, elem_of_app.
-    { revert Hnodup; rewrite /reqlist fmap_app omap_app; cbn; eauto. }
-    des; [left | right; apply elem_of_cons; right]; ss.
-  Qed.
-
-  Lemma reqlist_None_Some tl rid stid e0 e1 e2 reqmap :
-    rid ∉ dom reqmap →
-    tl !! stid = Some (e0, None) →
-    reqmap_tl tl ⊆ reqmap →
-    reqmap_tl (<[stid := (e1, Some (rid, e2))]> tl) ⊆ <[rid := e2]> reqmap.
-  Proof.
-    intros Hfresh Hin; rewrite /reqmap_tl /reqlist.
-    eapply elem_of_list_split_length in Hin as [tl1 [tl2 [-> Hlen]]].
-    rewrite -(Nat.add_0_r stid); subst stid; rewrite insert_app_r /=.
-    rewrite ?fmap_app ?omap_app; cbn; intros Hsub.
-    eapply map_subseteq_spec; intros i x Hi.
-    destruct (decide (i = rid)).
-    { subst.
-      rewrite list_to_map_app list_to_map_cons lookup_union lookup_insert in Hi.
-      set (m1 := list_to_map (omap id tl1.*2) : gmap nat (bool * jobID)).
-      destruct (m1 !! rid) eqn : Hm1; ss.
-      { exfalso; apply elem_of_dom_2 in Hm1; subst m1.
-        apply Hfresh. eapply elem_of_weaken; eauto.
-        apply subseteq_dom; etrans; last apply Hsub.
-        rewrite list_to_map_app; apply map_union_subseteq_l.
-      }
-      rewrite Hm1 left_id in Hi; clarify; rewrite lookup_insert //.
-    }
-    rewrite lookup_insert_ne //.
-    rewrite list_to_map_app list_to_map_cons lookup_union lookup_insert_ne // in Hi.
-    rewrite -lookup_union -list_to_map_app in Hi.
-    eapply lookup_weaken; eauto.
-  Qed. *)
-
-
-  (* Lemma NoDup_reqlist tl :
-    NoDup (reqlist_all tl).*1.*2 →
-    NoDup (omap (λ '(b, rid, jid), if b : bool then Some (rid, jid) else None) (reqlist_all tl)).*1.
-  Proof.
-    induction tl as [|[[??][[[[|]?]?]|]]]; first (ii; ss; econs); eauto.
-    { rewrite /reqlist_all fmap_cons; cbn. intros Hnodup; inv Hnodup.
-      econs; eauto. intros [[? ?] [? Hin%elem_of_list_omap]]%elem_of_list_fmap_2.
-      destruct Hin as [[[[|] ?] ?] [Hin' Hin]]; ss; clarify.
-      eapply H4. eapply (elem_of_list_fmap_1 fst) in Hin'; ss.
-      eapply (elem_of_list_fmap_1 snd) in Hin'; ss.
-    }
-    { rewrite /reqlist_all fmap_cons; cbn. intros Hnodup; inv Hnodup.
-      eapply IHtl; eauto.
-    }
-  Qed.
-
-  Lemma delete_lookup_reqmap tl stid e e0 b rid jid i :
-    tl !! stid = Some (e0, Some (b, rid, jid)) →
-    i ≠ rid →
-    reqmap (<[stid := (e, None)]> tl) !! i = (reqmap tl) !! i.
-  Proof.
-    intros Hin; eapply lookup_lt_Some in Hin as Hlen; revert Hin.
-    intros [tl1 [tl2 [-> ->]]]%elem_of_list_split_length Hneq.
-    rewrite -(Nat.add_0_r (length tl1)) insert_app_r /= /reqmap /reqlist_all.
-    rewrite ?fmap_app ?omap_app; destruct b; eauto; cbn.
-    { rewrite ?list_to_map_app list_to_map_cons.
-      set (m1 := list_to_map _). set (m2 := list_to_map _).
-      destruct (m1 !! i) eqn : Hin1.
-      { rewrite ?lookup_union Hin1 lookup_insert_ne //. }
-      rewrite ?lookup_union Hin1 lookup_insert_ne //.
-    }
-  Qed.
-
-  Lemma delete_reqmap tl stid e0 e1 b rid jid :
-    NoDup (reqlist_all tl).*1.*2 →
-    tl !! stid = Some (e0, Some (b, rid, jid)) →
-    delete rid (reqmap tl) = reqmap (<[stid := (e1, None)]> tl).
-  Proof.
-    intros Hdup Hstid; apply lookup_lt_Some in Hstid as Hlen.
-    apply map_eq; intros i; destruct (decide (i = rid)); subst.
-    { rewrite lookup_delete.
-      eapply elem_of_list_split_length in Hstid as [tl1 [tl2 [-> Htl]]].
-      rewrite -(Nat.add_0_r stid); subst stid. rewrite insert_app_r /=.
-      rewrite /reqmap /reqlist_all fmap_app omap_app; cbn.
-      rewrite (not_elem_of_list_to_map_1) //.
-      intros Hin; eapply elem_of_list_fmap_2 in Hin as [[rid' jid'] [EQ Hin]]; ss; clarify.
-      eapply elem_of_list_omap in Hin as [[[[|] rid2] jid2] [Hin ?]]; ss; clarify.
-      rewrite -omap_app -fmap_app in Hin.
-      revert Hdup; rewrite /reqlist_all.
-      rewrite cons_app Permutation_app_swap_app; cbn.
-      intros Hnodup; inv Hnodup; eapply H4, elem_of_list_fmap; exists (true, rid'); split; ss.
-      eapply elem_of_list_fmap; eexists (_, _, jid'); split; ss.
-    }
-    rewrite lookup_delete_ne //.
-    rewrite (delete_lookup_reqmap tl stid _ e0 b rid jid i) //.
-  Qed.
-
-  Lemma insert_reqmap_id tl stid e0 e1 o :
-    tl !! stid = Some (e0, o) →
-    reqmap tl = reqmap (<[stid := (e1, o)]> tl).
-  Proof.
-    intros Hin; eapply lookup_lt_Some in Hin as Hlen.
-    eapply elem_of_list_split_length in Hin as [tl1 [tl2 [-> ->]]].
-    rewrite -(Nat.add_0_r (length tl1)) insert_app_r /=.
-    rewrite /reqmap /reqlist_all ?fmap_app ?omap_app //.
-  Qed.
-
-  Lemma reqmap_lookup tl stid e (b : bool) rid jid :
-    NoDup (reqlist_all tl).*1.*2 →
-    tl !! stid = Some (e, Some (b, rid, jid)) →
-    reqmap tl !! rid = if b then Some jid else None.
-  Proof.
-    intros Hnodup Hin; eapply lookup_lt_Some in Hin as Hlen.
-    eapply elem_of_list_split_length in Hin as [tl1 [tl2 [-> ->]]].
-    rewrite /reqmap /reqlist_all ?fmap_app ?omap_app; cbn; destruct b.
-    { rewrite list_to_map_app list_to_map_cons lookup_union.
-      set (m1 := list_to_map _). set (m2 := list_to_map _).
-      destruct (m1 !! rid) eqn : Hm1.
-      { subst m1; eapply elem_of_list_to_map_2, elem_of_list_omap in Hm1.
-        destruct Hm1 as [[[[|] ?] ?] [Hin%elem_of_list_omap ?]]; ss; clarify.
-        destruct Hin as [[[[[|] ?] ?]|] [Hin ?]]; ss; clarify.
-        revert Hnodup; rewrite /reqlist_all ?fmap_app omap_app; cbn.
-        rewrite cons_app Permutation_app_swap_app; cbn.
-        intros Hnodup; inv Hnodup; exfalso; apply H4.
-        eapply elem_of_list_fmap; exists (true, rid); split; ss.
-        eapply elem_of_list_fmap; exists (true, rid, j); split; ss.
-        eapply elem_of_app; left; eapply elem_of_list_omap; eexists (Some (_, _, _)); eauto.
-      }
-      rewrite lookup_insert //.
-    }
-    rewrite -?omap_app -?fmap_app.
-    eapply not_elem_of_list_to_map; intros Hin.
-    eapply elem_of_list_fmap_2 in Hin as [[? ?] [EQ Hin]]; ss; clarify.
-    eapply elem_of_list_omap in Hin as [[[[|] ?] ?] [Hin ?]]; ss; clarify.
-    eapply elem_of_list_omap in Hin as [[[[[|] ?] ?]|] [Hin ?]]; ss; clarify.
-    revert Hnodup; rewrite /reqlist_all cons_app Permutation_app_swap_app; cbn.
-    intros Hinv; inv Hinv; eapply H4.
-    eapply elem_of_list_fmap; eexists (true, _); split; ss.
-    eapply elem_of_list_fmap; eexists (true, _, _); split; ss.
-    eapply elem_of_list_omap; eexists (Some (_, _, _)); split; ss; eauto.
-  Qed.
-
-  Lemma fresh_reqmap tl stid e0 e1 rid jid :
-    tl !! stid = Some (e0, None) →
-    rid ∉ dom (reqmap tl) →
-    <[rid := jid]> (reqmap tl) = reqmap (<[stid := (e1, Some (true, rid, jid))]> tl).
-  Proof.
-    intros Hstid Hrid; pose proof Hstid as Hstid'.
-    apply elem_of_list_split_length in Hstid' as [tl1 [tl2 [-> ->]]].
-    rewrite -(Nat.add_0_r (length tl1)) insert_app_r /=.
-    eapply map_eq; intros i; destruct (decide (i = rid)); subst.
-    { rewrite lookup_insert.
-      rewrite /reqmap /reqlist_all ?fmap_app ?omap_app; cbn; rewrite ?list_to_map_app.
-      rewrite list_to_map_cons; set (m1 := list_to_map _); set (m2 := list_to_map _).
-      rewrite ?lookup_union; destruct (m1 !! rid) eqn : Hm1; cycle 1.
-      { rewrite lookup_insert //. }
-      exfalso; apply Hrid; rewrite /reqmap /reqlist_all fmap_app ?omap_app; cbn.
-      rewrite list_to_map_app dom_union elem_of_union; left.
-      eapply elem_of_dom; rewrite Hm1 //.
-    }
-    rewrite lookup_insert_ne //.
-    rewrite /reqmap /reqlist_all ?fmap_app ?omap_app; cbn; rewrite ?list_to_map_app.
-    rewrite list_to_map_cons; set (m1 := list_to_map _); set (m2 := list_to_map _).
-    rewrite ?lookup_union; destruct (m1 !! i) eqn : Hm1.
-    { rewrite lookup_insert_ne //. }
-    rewrite lookup_insert_ne //.
-  Qed.
-
-  Lemma dom_reqmap tl :
-    ∀ i, i ∈ dom (reqmap tl) → i ∈ (reqlist_all tl).*1.*2.
-  Proof.
-    induction tl as [|[e [[[[|]?]?]|]]].
-    { rewrite /reqmap /reqlist_all. intros i; rewrite dom_empty; set_solver. }
-    { rewrite /reqmap /reqlist_all. intros i; cbn; rewrite dom_insert elem_of_union.
-      rewrite elem_of_cons; set_solver.
-    }
-    { intros i; cbn. set_solver. }
-    { intros i; cbn. set_solver. }
-  Qed. *)
+  Definition join_pend (arg : Any.t) stid ktr : itree lmodE Any.t :=
+    tau;;
+    x <- ⇓cris (⇓sb(false, wmask_and msk wmask_all, SchI.scopes)
+      (⇓smod(false, sp_none) (
+        'arg : () <- (arg↓)?;;
+        x_3 <- iterC (λ _ : (),
+          'x_1 : thpool <- cgetU SchI.v_ths;;
+          match x_1 !! stid with
+          | Some (_, Some rv) => Ret (inr (Some rv))
+          | Some (_, None) =>
+              '() : _ <- ccallU SchHdr.yield tt;; Ret (inl ())
+          | None => Ret (inr None)
+          end
+        ) ();;
+        Ret (x_3↑))));;
+    ktr x.
 
   Definition helpee_pend_s
-      (tid_cur : nat) (j : jobID) k
+      (j : jobID) k
       (fspo : option fspec) (x_fsp : fspec_option_meta fspo)
       : itree lmodE Any.t :=
     tau;;
@@ -648,7 +533,7 @@ Section Helping.
      (k r).
 
   Definition helpee_pend_t
-      (tid_cur tid_stid_cur : nat) (j : jobID) k
+      (tid_stid_cur : nat) (j : jobID) k
       (fspo : option fspec) (x_fsp : fspec_option_meta fspo)
       : itree lmodE Any.t :=
     tau;;
@@ -658,10 +543,13 @@ Section Helping.
     ));; (k r).
 
   Inductive help_rel : itree lmodE Any.t → itree lmodE Any.t → option (nat * (bool * jobID)) → Prop :=
-  | help_rel_eq itr_s itr_t itr img msk scp :
-      itr_t = itr_s →
-      itr_s = ModTr.trans (SB.sandbox img msk scp itr) →
+  | help_rel_ret ret : help_rel (Ret ret) (Ret ret) None
+  | help_rel_eq itr_s itr_t (k_s k_t : Any.t → _) itr img msk scp :
+      itr_t = ModTr.trans (SB.sandbox img msk scp itr) >>= k_t →
+      itr_s = ModTr.trans (SB.sandbox img msk scp itr) >>= k_s →
       scp ## (SchI.scopes ++ HelpingOff.scopes mn) →
+      (∀ ret, itr ≠ Ret ret) →
+      (∀ ret, help_rel (k_s ret) (k_t ret) None) →
       help_rel itr_s itr_t None
   | help_rel_loop itr_s itr_t ktr_t ktr_s x :
       itr_t = (tau;;
@@ -676,8 +564,8 @@ Section Helping.
         ktr_s x_) →
       (∀ ret, help_rel (ktr_s ret) (ktr_t ret) None) →
       help_rel itr_s itr_t None
-  | help_rel_helpee_done tid_cur tid jid itr_s itr_t x k_s k_t :
-      itr_t = helpee_pend_t tid_cur tid jid k_t (sp SchHdr.yield) x →
+  | help_rel_helpee_done tid jid itr_s itr_t x k_s k_t :
+      itr_t = helpee_pend_t tid jid k_t (sp SchHdr.yield) x →
       itr_s = (tau;;
         x_ <- ⇓cris(⇓sb(true, wmask_all, HelpingOn.scopes mn)
           (x_2 <- HoareCall_epilogue (sp SchHdr.yield) x (()↑);;
@@ -685,17 +573,40 @@ Section Helping.
         k_s x_) →
       (∀ ret, help_rel (k_s ret) (k_t ret) None) →
       help_rel itr_s itr_t (Some (tid, (false, jid)))
-  | help_rel_helpee_pend tid jid itr_s itr_t tid_cur k_s k_t x_fsp :
-      itr_s = helpee_pend_s tid_cur jid k_s (sp SchHdr.yield) x_fsp →
-      itr_t = helpee_pend_t tid_cur tid jid k_t (sp SchHdr.yield) x_fsp →
+  | help_rel_helpee_pend tid jid itr_s itr_t k_s k_t x_fsp :
+      itr_s = helpee_pend_s jid k_s (sp SchHdr.yield) x_fsp →
+      itr_t = helpee_pend_t tid jid k_t (sp SchHdr.yield) x_fsp →
       (∀ ret, help_rel (k_s ret) (k_t ret) None) →
       help_rel itr_s itr_t (Some (tid, (true, jid)))
   | help_rel_call itr_s itr_t ktr_t ktr_s ktr_t1 ktr_s1 ctx rs fn arg :
+      Some fn ∈ List.map fst (Mod.fnsems ((HelpingOn.t mn jobs sp) ★ (CFilter.filter msk SchI.t))) →
+      Mod.wf ((HelpingOn.t mn jobs sp ★ CFilter.filter msk SchI.t) ★ ctx) →
       prog_t ctx rs fn = Some ktr_t →
       prog_s ctx rs fn = Some ktr_s →
       itr_t = ktr_t arg >>= ktr_t1 →
       itr_s = ktr_s arg >>= ktr_s1 →
       (∀ ret, help_rel (ktr_s1 ret) (ktr_t1 ret) None) →
+      help_rel itr_s itr_t None
+  | help_rel_inner_spawn itr_s itr_t (arg : Any.t) ktr_s ktr_t :
+      itr_t = inner_spawn_pend arg ktr_t →
+      itr_s = inner_spawn_pend arg ktr_s →
+      (∀ ret, help_rel (ktr_s ret) (ktr_t ret) None) →
+      help_rel itr_s itr_t None
+  | help_rel_join itr_s itr_t (arg : Any.t) ktr_s ktr_t tid :
+      itr_t = join_pend arg tid ktr_t →
+      itr_s = join_pend arg tid ktr_s →
+      (∀ ret, help_rel (ktr_s ret) (ktr_t ret) None) →
+      help_rel itr_s itr_t None
+  | help_rel_terminate itr_s itr_t ktr_s ktr_t :
+      itr_s =
+        (x <- ⇓cris (⇓sb( false, wmask_and msk wmask_all, SchI.scopes)
+          (⇓smod( false, sp_none) (x_ <- Sch.terminate;; Ret x_↑)));;
+        ktr_s x) →
+      itr_t =
+        (x <- ⇓cris (⇓sb( false, wmask_and msk wmask_all, SchI.scopes)
+          (⇓smod( false, sp_none) (x_ <- Sch.terminate;; Ret x_↑)));;
+        ktr_t x) →
+      (∀ ret, help_rel (ktr_s ret) (ktr_t ret) None) →
       help_rel itr_s itr_t None.
 
   Lemma gsim_Yield_tgt r g RR p_s p_t tid_s tid_t tp_s tp_t
@@ -765,8 +676,7 @@ Section Helping.
           (ModTr.alist_encode ((HelpingOn.v_reqs mn, reqs)
           :: (SchI.v_ths, (ths ↑)) :: (SchI.v_tid, (tid_cur_t ↑)) :: st_ctx))
           (res↑))).
-  Admitted.
-  (* Proof.
+  Proof.
     intros Hres Hlen_s Hlen_t Hk1 Hk2; revert Hk1; rewrite yield_unfold; ired.
     revert res Hres.
     gcofix CIH.
@@ -820,9 +730,9 @@ Section Helping.
     destruct (msk_c _); cycle 1; ss.
     { step_l; ss. }
     step_l; step_r; norm_l; norm_r; rewrite {1 3}/LMod.prog /=; destruct (dec _ _) as [e|e]; ss.
-    { inv e; exfalso; apply yield_run_neq; eauto. }
+    { inv e; exfalso; eapply yield_run_neq; eauto. }
     clear e; destruct (dec _ _) as [e|e].
-    { ss. inv e; exfalso; apply yield_help_neq; eauto. }
+    { ss. inv e; exfalso; eapply yield_help_neq; eauto. }
     ss; clear e. norm_l. rewrite list_insert_insert. ss.
     norm_r. rewrite list_insert_insert. ss.
 
@@ -912,7 +822,7 @@ Section Helping.
     rewrite list_insert_insert. ired.
     rewrite ?interpV_ret. ired.
     eapply gpaco7_mon; first eapply Hk3; eauto.
-  Qed. *)
+  (*SLOW*)Admitted.
 
   Lemma gsim_Yield_both r g RR p_s p_t tid_s tid_t tp_s tp_t
       img_c msk_c scp_c k_s k_t (k_s1 k_t1 : Any.t → itree _ Any.t) ctx rs
@@ -982,197 +892,19 @@ Section Helping.
           (ModTr.alist_encode ((HelpingOn.v_reqs mn, reqs)
           :: (SchI.v_ths, (ths ↑)) :: (SchI.v_tid, (tid_cur_t ↑)) :: st_ctx))
           (res↑))).
-  Admitted.
-  (* Proof.
-    intros Hres Hlen_s Hlen_t Hk1 Hk2; revert Hk1; rewrite yield_unfold; ired.
-    revert res Hres.
-    gcofix CIH.
-    intros res Hres Hk1.
-    replace_r; [rewrite interpV_tau //|].
-    eapply gsim_tau_tgt; [rewrite list_lookup_insert //|rewrite list_insert_insert].
-    rewrite interpV_tau.
-    eapply gsim_tau_src; [rewrite list_lookup_insert //|rewrite list_insert_insert].
-    zprogress.
-    replace_r; [rewrite interpV_bind interpV_trigger //=|]; ired.
-    eapply gsim_Choose_tgt; [rewrite list_lookup_insert // length_insert //|].
-    intros [[|]|]; cycle 1; rewrite list_insert_insert.
-    {
-      ired. rewrite interpV_bind interpV_trigger //=; ired.
-      eapply gsim_Choose_src; [rewrite list_lookup_insert //|].
-      exists (Some false); rewrite list_insert_insert.
-      rewrite yield_unfold; ired.
-      guclo flagC_spec; econs; [instantiate (1:=p_s)|instantiate (1:=p_t)|].
-      { destruct p_s as [[|]|]; rr; ss; eauto. }
-      { destruct p_t as [[|]|]; rr; ss; eauto. }
-      gbase. eapply CIH; eauto.
-    }
-    {
-      clear CIH.
-      ired. rewrite interpV_bind interpV_trigger //=; ired.
-      eapply gsim_Choose_src; [rewrite list_lookup_insert //|].
-      exists (None); rewrite list_insert_insert. ired.
-      eapply gpaco7_mon; eauto.
-    }
-    ired. rewrite interpV_bind interpV_trigger //=; ired.
-    eapply gsim_Choose_src; [rewrite list_lookup_insert //|].
-    exists (Some true); rewrite list_insert_insert. ired.
-
-    iter_l; rewrite list_lookup_insert //=; step_l; norm_l.
-    rewrite list_insert_insert.
-    iter_r; rewrite list_lookup_insert //=; step_r; norm_r.
-    rewrite list_insert_insert.
-
-    rewrite !HoareCall_unfold; ired.
-    eapply gsim_HoareCall_prologue_both;
-      [rewrite list_lookup_insert //
-      |rewrite list_lookup_insert //
-      |ss
-      |].
-    intros res1 [x arg] Hres1.
-    rewrite ?list_insert_insert. ired.
-
-    iter_l; rewrite list_lookup_insert //=.
-    iter_r; rewrite list_lookup_insert //=.
-    destruct (msk_c _); cycle 1; ss.
-    { step_l; ss. }
-    step_l; step_r; norm_l; norm_r; rewrite {1 3}/LMod.prog /=; destruct (dec _ _) as [e|e]; ss.
-    { inv e; exfalso; apply yield_run_neq; eauto. }
-    clear e; destruct (dec _ _) as [e|e].
-    { ss. inv e; exfalso; apply yield_help_neq; eauto. }
-    ss; clear e. norm_l. rewrite list_insert_insert. ss.
-    norm_r. rewrite list_insert_insert. ss.
-
-    rewrite /ModTr.trans_ktree /ModTr.trans /SB.sandbox_body /SB.sandbox /SModTr.trans /=.
-    eapply gsim_tau_tgt; [rewrite list_lookup_insert //|rewrite list_insert_insert].
-    eapply gsim_tau_src; [rewrite list_lookup_insert //|rewrite list_insert_insert].
-    rewrite /SchI.yield /cfunU.
-    destruct (arg ↓) eqn : Harg; cycle 1.
-    { ss; iter_l; rewrite list_lookup_insert //=.
-      destruct (excluded_middle_informative _); step_l; ss.
-    }
-    ss. ired. rewrite /cgetU /=. ired.
-
-    replace_r; [rewrite interpV_bind interpV_vis //|]. ired.
-    eapply gsim_sGet_tgt;
-      [rewrite list_lookup_insert //=| ss | ].
-    esplits; eauto. rewrite list_insert_insert.
-
-    replace_l; [rewrite interpV_bind interpV_vis //|]. ired.
-    eapply gsim_sGet_src;
-      [rewrite list_lookup_insert //=| ss | ].
-    esplits; eauto. rewrite list_insert_insert.
-    rewrite ?interpV_ret. ired. hss. ired. rewrite ?interpV_ret. ired. hss. ired.
-
-    iter_l; rewrite list_lookup_insert //=. step_l; norm_l.
-    rewrite list_insert_insert.
-    iter_r; rewrite list_lookup_insert //=; step_r; norm_r.
-    rewrite list_insert_insert.
-
-    iter_l; rewrite list_lookup_insert //=. step_l; norm_l.
-    rewrite list_insert_insert.
-    iter_r; rewrite list_lookup_insert //=; step_r; norm_r.
-    rewrite list_insert_insert. ired.
-
-    replace_r; [rewrite interpV_bind interpV_vis //|]. ired.
-    eapply gsim_sGet_tgt;
-      [rewrite list_lookup_insert //=| ss | ].
-    esplits; eauto. rewrite list_insert_insert.
-
-    replace_l; [rewrite interpV_bind interpV_vis //|]. ired.
-    eapply gsim_sGet_src;
-      [rewrite list_lookup_insert //=| ss | ].
-    esplits; eauto. rewrite list_insert_insert.
-    rewrite ?interpV_ret. ired. hss. ired. rewrite ?interpV_ret. ired. hss. ired.
-
-    destruct (ths !! tid_cur_s) as [[stid_cur_s reto_s]|] eqn : Htid_cur_s; cycle 1.
-    { rewrite Htid_cur_s /=.
-      ss; iter_l; rewrite list_lookup_insert //=.
-      destruct (excluded_middle_informative _); step_l; ss.
-    }
-    rewrite Htid_cur_s //=.
-    destruct (decide (stid_cur_s = tid_s)); subst; cycle 1.
-    { ss; iter_l; rewrite list_lookup_insert //=.
-      destruct (excluded_middle_informative _); step_l; ss.
-    }
-    hexploit Hk2; eauto; clear Hk2; intros [? [Htid_t Hk2]].
-    rewrite Htid_t; case_decide; clarify; ired.
-
-    replace_r; [rewrite interpV_bind interpV_trigger //=|]; ired.
-    eapply gsim_Choose_tgt; [rewrite list_lookup_insert // length_insert //|].
-    intros [[mtidn stidn] Hmtidn]; rewrite list_insert_insert; ired; ss.
+  Proof.
+    intros Hres Hlen_s Hlen_t Hk1 Hk2.
+    eapply gsim_Yield_tgt; eauto.
+    rewrite {1}yield_unfold. ired.
+    replace_l; [rewrite interpV_tau //|]; ired.
+    eapply gsim_tau_src; [rewrite list_lookup_insert //|]. rewrite list_insert_insert.
 
     replace_l; [rewrite interpV_bind interpV_trigger //=|]; ired.
-    eapply gsim_Choose_src; [rewrite list_lookup_insert // length_insert //|].
-    specialize (Hk2 mtidn stidn Hmtidn); destruct Hk2 as [mtidn_s [stidn_s [Htid_s Hk3]]].
-    unshelve eexists.
-    { exists (mtidn_s, stidn_s); ss; eauto. }
-    rewrite list_insert_insert; ired; ss.
+    eapply gsim_Choose_src; [rewrite list_lookup_insert //|].
+    exists (None); rewrite list_insert_insert. ired.
 
-    iter_l; rewrite list_lookup_insert //=. step_l; norm_l.
-    rewrite list_insert_insert. hss.
-    iter_l; rewrite list_lookup_insert //=. step_l; norm_l.
-    rewrite list_insert_insert. ired.
-    iter_r; rewrite list_lookup_insert //=; step_r; norm_r.
-    rewrite list_insert_insert. hss.
-    iter_r; rewrite list_lookup_insert //=; step_r; norm_r.
-    rewrite list_insert_insert. ired.
-    rewrite ?ModTr.alist_encode_decode /alist_upd /=; destruct (dec _ _); clarify.
-
-    iter_l; rewrite list_lookup_insert //=. step_l; norm_l.
-    rewrite list_insert_insert. hss.
-    iter_l; rewrite list_lookup_insert //=. step_l; norm_l.
-    rewrite list_insert_insert. ired.
-    iter_r; rewrite list_lookup_insert //=. step_r; norm_r.
-    rewrite list_insert_insert. hss.
-    iter_r; rewrite list_lookup_insert //=. step_r; norm_r.
-    rewrite list_insert_insert. ired.
-    rewrite ?interpV_ret. ired.
-    eapply gpaco7_mon; first eapply Hk3; eauto.
-  Qed. *)
-
-  (* Lemma gsim_no_help RR r g p_s p_t rs tl img_c msk_c scp_c (ths : list (nat * option SAny.t))
-      (mtid stid : nat) fn args k st_ctx ctx :
-    fn ≠ Helping.help mn →
-    fn ≠ Helping.run mn →
-    tl !! stid =
-    Some (⇓cris (⇓sb( img_c, msk_c, scp_c) (x <- trigger (Call fn args);; k x)),
-          ⇓cris (⇓sb( img_c, msk_c, scp_c) (x <- trigger (Call fn args);; k x)), None) →
-    gpaco7 _gsim (cpn7 _gsim) r g (Any.t * Any.t)%type (Any.t * Any.t)%type RR p_s p_t
-      (LModTr.interp_stateE Any.t
-        (iterV (LModTr.handle_callE (prog_s ctx rs)) (stid, fst ∘ fst <$> tl))
-        (Any.pair
-          (ModTr.alist_encode ((SchI.v_ths, ths ↑) :: (SchI.v_tid, mtid ↑) :: st_ctx))
-          (rs ↑)))
-      (LModTr.interp_stateE Any.t
-        (iterV (LModTr.handle_callE (prog_t ctx rs)) (stid, snd ∘ fst <$> tl))
-        (Any.pair
-          (ModTr.alist_encode ((HelpingOn.v_reqs mn, (reqmap tl) ↑)
-          :: (SchI.v_ths, ths ↑) :: (SchI.v_tid, mtid ↑) :: st_ctx)) rs ↑)).
-  Proof.
-    intros Hfnhelp Hfnrun Hstid. eapply lookup_lt_Some in Hstid as Hstidlen.
-    iter_l; iter_r; rewrite ?list_lookup_fmap Hstid /=.
-    destruct (msk_c fn); ss; [|step_l; ss].
-    step_l; step_r.
-    hexploit (prog_fn fn); eauto; intros [[-> ?]|[[-> ?]|[EQ Hfn]]]; ss. rewrite -EQ; clear EQ.
-    destruct Hfn as [[-> ->]|Hfn].
-    {
-      ss. norm_l; norm_r. rewrite /yield.
-      eapply gsim_tau_src; [rewrite list_lookup_insert // length_fmap //|].
-      eapply gsim_tau_tgt; [rewrite list_lookup_insert // length_fmap //|].
-      rewrite ?list_insert_insert.
-
-      rewrite /SchI.yield /cfunU /=.
-      destruct (args ↓) as [arg|] eqn : Hargs; cycle 1.
-      { ss. ired. rewrite interpV_bind interpV_vis /=; ired.
-        eapply gsim_Take_src; [rewrite list_lookup_insert // length_fmap //|]. ss.
-      }
-      destruct arg; clear Hargs; ss. ired.
-      rewrite
-    } *)
-
-  Ltac unfold_trans :=
-    rewrite /ModTr.trans_ktree /SB.sandbox_body /SB.sandbox
-      /ModTr.trans /SModTr.trans_ktree /SModTr.trans /=.
+    eapply Hk1.
+  Qed.
 
   Theorem helping_onoff_correct :
     ctx_refines (mod_off, emp%I) (mod_on, emp%I).
@@ -1217,7 +949,7 @@ Section Helping.
     rewrite /SB.sandbox_body /=.
     ginit. guclo bindC_spec. econs; cycle 1.
     { instantiate (1:=λ r_s r_t, r_s.2 = r_t.2). ii; gstep; ss. subst; econs; econs; ss. }
-
+    unfold_trans.
     (* Start coinduction *)
     rewrite /HelpingOff.t /HelpingOn.t /SchI.t; unseal CRIS; ss.
     set (st_src := (_, _) :: _) at 1.
@@ -1247,7 +979,20 @@ Section Helping.
       }
       intros ???? [-> In]%list_lookup_singleton_Some; clarify.
       split; ss.
-      eapply help_rel_eq; eauto.
+      ides (f arg).
+      { rewrite ?interpV_ret; eapply help_rel_ret. }
+      { eapply help_rel_eq; eauto.
+        { instantiate (1:=λ a, Ret a). ired. refl. }
+        { instantiate (1:=λ a, Ret a). ired. refl. }
+        { ii; clarify. }
+        apply help_rel_ret.
+      }
+      { eapply help_rel_eq; eauto.
+        { instantiate (1:=λ a, Ret a). ired. refl. }
+        { instantiate (1:=λ a, Ret a). ired. refl. }
+        { ii; clarify. }
+        apply help_rel_ret.
+      }
     }
     generalize st_src, st_tgt, tp_src, tp_tgt.
     clear st_src st_tgt tp_src tp_tgt f imgf mskf scpf FIND arg Hscp.
@@ -1453,7 +1198,7 @@ Section Helping.
       exists None; rewrite list_insert_insert.
       ired. rewrite ?interpV_ret; ired. rewrite ?interpV_ret; ired.
 
-      guclo flagC_spec; econs; try instantiate (1:=smj_bot); eauto using smj_le_bot.
+      eapply gsim_flag.
 
       gbase. eapply (CIH res1); eauto.
       eexists (<[stid := (_, _, None)]> tl); ss; esplits; eauto.
@@ -1470,7 +1215,7 @@ Section Helping.
     apply lookup_lt_Some in Htid as Hstid_cur_length.
     pose proof Htid as Htid'.
     apply Hlookup in Htid' as [Hcase _].
-    inv Hcase; cycle 1.
+    inv Hcase; cycle 2.
     { (* Done helper case *)
       eapply lookup_lt_Some in Htid as Htidlen.
       iter_l; iter_r; rewrite ?list_lookup_fmap Htid /=.
@@ -1522,7 +1267,7 @@ Section Helping.
 
     { (* call case *)
       eapply lookup_lt_Some in Htid as Htidlen.
-      revert H2 H3.
+      revert H4 H5.
       destruct (decide (fn = Helping.run mn)); subst.
       { (* Helping.run *)
         rewrite {1 2}/LMod.prog ?alist_find_map_snd /=.
@@ -1545,7 +1290,7 @@ Section Helping.
         esplits; eauto.
         { des_ifs; destruct (dec _ _); clarify. }
         rewrite list_insert_insert.
-        
+
         replace_r; [rewrite interpV_bind //|]. ired.
         eapply gsim_s_cput_tgt; [rewrite list_lookup_insert // length_fmap //| |]; s.
         { rewrite String.eqb_refl //. }
@@ -1831,7 +1576,7 @@ Section Helping.
             |].
           esplits; eauto.
           rewrite list_insert_insert.
-          
+
           iter_l; rewrite list_lookup_insert //=; [|rewrite length_fmap //].
           step_l; norm_l. rewrite list_insert_insert.
           iter_l; rewrite list_lookup_insert //=; [|rewrite length_fmap //].
@@ -2089,7 +1834,7 @@ Section Helping.
         ired. rewrite interpV_ret. ired. rewrite ?interpV_ret. ired.
 
         rewrite /alist_upd /=; destruct (dec _ _); ss; clear e.
-        guclo flagC_spec; econs; first instantiate (1:=smj_bot); eauto using smj_le_bot.
+        apply gsim_flag.
         gbase. eapply (CIH res1); eauto.
         set (i_helpee := tau;; _).
         eexists (<[stid := (ktr_s1 () ↑, ktr_t1 () ↑, None)]>
@@ -2148,8 +1893,7 @@ Section Helping.
         rewrite ?list_insert_insert.
 
         destruct ((wmask_and msk wmask_all) fn) eqn : Hfn; cycle 1.
-        {
-          iter_l; rewrite list_lookup_insert /=; [rewrite Hfn /=|rewrite length_fmap //].
+        { iter_l; rewrite list_lookup_insert /=; [rewrite Hfn /=|rewrite length_fmap //].
           step_l; ss.
         }
 
@@ -2158,17 +1902,70 @@ Section Helping.
         step_l; step_r. norm_l; norm_r.
         destruct (prog_s ctx rs fn) eqn : Hfn_s; cycle 1.
         { step_l; ss. }
-        (* eapply prog_s_prog_t in Hfn_s as Hfn_t. *)
         destruct (prog_t ctx rs fn) eqn : Hfn_t; cycle 1.
         { eapply prog_s_prog_t in Hfn_s as Hfn_t'; des; clarify. }
         norm_l; norm_r.
         rewrite !list_insert_insert.
-        iter_l; it
-        admit.
+        gstep; econs; eapply gsim_progress; try instantiate (1:=smj_bot); eauto using smj_le_bot.
+        gbase.
+        eapply (CIH rs); eauto.
+        eexists (<[stid := (_, _, None)]> tl); ss; esplits; eauto.
+        { rewrite list_fmap_insert //=. }
+        { rewrite list_fmap_insert //=. }
+        { eapply reqmap_rel_id; eauto. }
+        { intros i1; destruct (decide (i1 = stid)); subst; cycle 1.
+          { intros ???; rewrite list_lookup_insert_ne //=; apply Hlookup. }
+          { rewrite list_lookup_insert; ii; clarify. split; ss.
+            destruct (decide (Some fn ∈
+              List.map fst (Mod.fnsems ((HelpingOn.t mn jobs sp) ★ (CFilter.filter msk SchI.t))))).
+            { eapply (help_rel_call _ _ _ _ _ _ ctx); eauto. intros ret; ss.
+              eapply help_rel_inner_spawn; eauto.
+              { rewrite /inner_spawn_pend; grind. instantiate (1:=ret); f_equal; grind.
+                repeat f_equal; extensionalities a; grind.
+              }
+              { rewrite /inner_spawn_pend; grind. f_equal; grind.
+                repeat f_equal; extensionalities a; grind.
+              }
+            }
+            hexploit (prog_fn_ctx fn ctx rs); eauto.
+            intros [Hs|[itr_ctx [img1 [msk1 [scp1 [Ht Hs]]]]]]; des; clarify.
+            rewrite Ht Hs in Hfn_t; inv Hfn_t; ss.
+            ides (itr_ctx args ↑).
+            { rewrite ?interpV_ret; ired.
+              eapply help_rel_inner_spawn; eauto.
+              { rewrite /inner_spawn_pend; grind. f_equal; grind.
+                repeat f_equal; extensionalities a; grind.
+              }
+              { rewrite /inner_spawn_pend; grind. f_equal; grind.
+                repeat f_equal; extensionalities a; grind.
+              }
+            }
+            { eapply (help_rel_eq); eauto.
+              i; ss.
+              eapply help_rel_inner_spawn; eauto.
+              { rewrite /inner_spawn_pend; grind. instantiate (1:=ret); f_equal; grind.
+                repeat f_equal; extensionalities a; grind.
+              }
+              { rewrite /inner_spawn_pend; grind. f_equal; grind.
+                repeat f_equal; extensionalities a; grind.
+              }
+            }
+            { eapply (help_rel_eq); eauto.
+              i; ss.
+              eapply help_rel_inner_spawn; eauto.
+              { rewrite /inner_spawn_pend; grind. instantiate (1:=ret); f_equal; grind.
+                repeat f_equal; extensionalities a; grind.
+              }
+              { rewrite /inner_spawn_pend; grind. f_equal; grind.
+                repeat f_equal; extensionalities a; grind.
+              }
+            }
+          }
+        }
       }
 
       destruct (decide (fn = SchHdr.spawn)); subst.
-      { (* SchI.inner_spawn *)
+      { (* SchI.spawn *)
         rewrite {1 2}/LMod.prog ?alist_find_map_snd /=.
         destruct (dec _ _) as [?|e]; ss; [inv e; clear e|clarify; clear e].
         destruct (dec _ _) as [e|e]; ss; [inv e; clear e|clarify; clear e].
@@ -2182,7 +1979,100 @@ Section Helping.
         zprogress.
 
         rewrite /cfunU.
-        admit.
+        destruct (arg ↓) as [[fn args]|] eqn : Harg; ss; ired; cycle 1.
+        { replace_l; [rewrite interpV_bind interpV_trigger //|].
+          eapply gsim_Take_src;
+            [rewrite list_lookup_insert // ?length_fmap //; repeat f_equal; grind
+            |intros x ?].
+          rewrite list_insert_insert; ss.
+        }
+        clear Harg.
+        rewrite /ccallU.
+
+        ired. replace_l; [rewrite interpV_bind //|]; ired.
+        eapply gsim_s_cgetU_src;
+          [rewrite list_lookup_insert // length_fmap //
+          |ss; rewrite String.eqb_refl //
+          |].
+        esplits; eauto.
+        rewrite list_insert_insert.
+
+        ired. replace_r; [rewrite interpV_bind //|]; ired.
+        eapply gsim_s_cgetU_tgt;
+          [rewrite list_lookup_insert // length_fmap //
+          |ss; rewrite String.eqb_refl //
+          |].
+        esplits; eauto.
+        rewrite list_insert_insert. ired.
+
+        iter_l. rewrite list_lookup_insert /=; [|rewrite length_fmap //]. step_l. norm_l.
+        rewrite list_insert_insert.
+        iter_r. rewrite list_lookup_insert /=; [|rewrite length_fmap //]. step_r. norm_r.
+        rewrite list_insert_insert. ired.
+        rewrite /SModTr.NativeSpawn; ired.
+
+        destruct ((wmask_and msk wmask_all) SchHdr._spawn) eqn : Hfn; cycle 1.
+        {
+          iter_l; rewrite list_lookup_insert /=; [rewrite Hfn /=|rewrite length_fmap //].
+          step_l; ss.
+        }
+
+        iter_l; rewrite ?list_lookup_insert /=; last rewrite ?length_fmap //. rewrite Hfn /=.
+        iter_r; rewrite ?list_lookup_insert /=; last rewrite ?length_fmap //. rewrite Hfn /=.
+        step_l; step_r. norm_l; norm_r.
+        destruct (prog_s ctx rs SchHdr._spawn) eqn : Hfn_s; cycle 1.
+        { step_l; ss. }
+        destruct (prog_t ctx rs SchHdr._spawn) eqn : Hfn_t; cycle 1.
+        { eapply prog_s_prog_t in Hfn_s as Hfn_t'; des; clarify. }
+        norm_l; norm_r.
+        rewrite !list_insert_insert. ired.
+
+        ired. replace_r; [rewrite interpV_bind //|]. ired.
+        eapply gsim_s_cput_tgt; s.
+        { rewrite lookup_app list_lookup_insert // length_fmap //. }
+        { ss. }
+        rewrite insert_app_l // ?length_insert ?length_fmap //.
+        rewrite /alist_upd /=; destruct (dec _ _) as [e|e]; ss; clarify; clear e.
+
+        ired. replace_l; [rewrite interpV_bind //|]. ired.
+        eapply gsim_s_cput_src; s.
+        { rewrite lookup_app list_lookup_insert // length_fmap //. }
+        { ss. }
+        rewrite insert_app_l // ?length_insert ?length_fmap //.
+        rewrite /alist_upd /=; destruct (dec _ _) as [e|e]; ss; clarify; clear e.
+        rewrite ?list_insert_insert.
+        rewrite ?interpV_ret. ired.
+
+        gstep; econs; eapply gsim_progress; try instantiate (1:=smj_bot); eauto using smj_le_bot.
+        gbase.
+        eapply (CIH rs); eauto.
+        eexists ((<[stid := (_, _, None)]> tl) ++ [(i (fn, args)↑, i0 (fn, args)↑, None)]); ss.
+        esplits; eauto.
+        { rewrite ?fmap_app list_fmap_insert //=. }
+        { rewrite ?fmap_app list_fmap_insert //=. }
+        { eapply reqmap_rel_append; eauto.
+          eapply reqmap_rel_id; eauto.
+        }
+        { intros i1; destruct (decide (i1 = length tl)); subst.
+          { intros ???; rewrite lookup_app_r // ?length_insert; try lia.
+            rewrite Nat.sub_diag /=; intros Heq; inv Heq.
+            split; ss.
+            eapply (help_rel_call _ _ _ _ (λ a, Ret a) (λ a, Ret a) ctx rs SchHdr._spawn); eauto.
+            { rewrite /HelpingOn.t /SchI.t; unseal CRIS; ss; set_solver. }
+            { grind. }
+            { grind. }
+            intros res; eapply help_rel_ret; eauto.
+          }
+          destruct (decide (i1 = stid)); subst.
+          { intros ???; rewrite -insert_app_l // list_lookup_insert // ?length_app; try lia.
+            intros EQ; clarify.
+          }
+          rewrite -insert_app_l // list_lookup_insert_ne //.
+          intros ??? [[Hilen Hi]|[??]]%lookup_snoc_Some; last clarify.
+          eapply Hlookup in Hi; des; split; eauto.
+          destruct no; eauto. des; eexists _, _; rewrite lookup_app_l //.
+          eapply lookup_lt_Some; eauto.
+        }
       }
 
       destruct (decide (fn = SchHdr.join)); subst.
@@ -2200,11 +2090,108 @@ Section Helping.
         zprogress.
 
         rewrite /cfunU.
-        admit.
+        destruct (arg ↓) as [?|] eqn : Harg; ss; ired; cycle 1.
+        { replace_l; [rewrite interpV_bind interpV_trigger //|].
+          eapply gsim_Take_src;
+            [rewrite list_lookup_insert // ?length_fmap //; repeat f_equal; grind
+            |intros x ?].
+          rewrite list_insert_insert; ss.
+        }
+        clear Harg.
+        (* gcofix CIH1. *)
+        rewrite unfold_iterC; ired.
+        rewrite {1 2}interpV_tau.
+        eapply gsim_tau_src; [rewrite list_lookup_insert // length_fmap //|].
+        eapply gsim_tau_tgt; [rewrite list_lookup_insert // length_fmap //|].
+        rewrite !list_insert_insert.
+
+        replace_l; [rewrite interpV_bind //|]. ired.
+        eapply gsim_s_cgetU_src; [rewrite list_lookup_insert // length_fmap //| |]; s.
+        { rewrite String.eqb_refl //. }
+        esplits; eauto.
+        rewrite ?list_insert_insert. ired.
+
+        replace_r; [rewrite interpV_bind //|]. ired.
+        eapply gsim_s_cgetU_tgt; [rewrite list_lookup_insert // length_fmap //| |]; s.
+        { rewrite String.eqb_refl //. }
+        esplits; eauto.
+        rewrite ?list_insert_insert. ired.
+
+        destruct (ths !! n3) as [[? [rv|]]|] eqn : Hret; rewrite Hret /=; ired.
+        { (* Join-return *)
+          rewrite ?interpV_ret; ired.
+          gstep; econs; eapply gsim_progress; try instantiate (1:=smj_bot); eauto using smj_le_bot.
+          gbase. eapply (CIH rs); eauto.
+          eexists (<[stid := (_, _, None)]> tl); esplits; eauto.
+          { rewrite list_fmap_insert //=. }
+          { rewrite list_fmap_insert //=. }
+          { eapply reqmap_rel_id; eauto. }
+          { intros i; destruct (decide (i = stid)); subst; cycle 1.
+            { intros ???; rewrite list_lookup_insert_ne //=; apply Hlookup. }
+            { rewrite list_lookup_insert; ii; clarify. }
+          }
+        }
+        { (* Join-loop *)
+          rewrite /ccallU.
+
+          iter_l. rewrite list_lookup_insert /=; [|rewrite length_fmap //]. step_l. norm_l.
+          rewrite list_insert_insert.
+          iter_r. rewrite list_lookup_insert /=; [|rewrite length_fmap //]. step_r. norm_r.
+          rewrite list_insert_insert. ired.
+
+          destruct ((wmask_and msk wmask_all) SchHdr.yield) eqn : Hfn; cycle 1.
+          { iter_l; rewrite list_lookup_insert /=; [rewrite Hfn /=|rewrite length_fmap //].
+            step_l; ss.
+          }
+
+          iter_l; rewrite ?list_lookup_insert /=; last rewrite ?length_fmap //. rewrite Hfn /=.
+          iter_r; rewrite ?list_lookup_insert /=; last rewrite ?length_fmap //. rewrite Hfn /=.
+          step_l; step_r. norm_l; norm_r.
+          destruct (prog_s ctx rs SchHdr.yield) eqn : Hfn_s; cycle 1.
+          { step_l; ss. }
+          destruct (prog_t ctx rs SchHdr.yield) eqn : Hfn_t; cycle 1.
+          { eapply prog_s_prog_t in Hfn_s as Hfn_t'; des; clarify. }
+          norm_l; norm_r.
+          rewrite !list_insert_insert. ired.
+          gstep; econs; eapply gsim_progress; try instantiate (1:=smj_bot); eauto using smj_le_bot.
+          gbase. eapply (CIH rs); eauto.
+          eexists (<[stid := (_, _, None)]> tl); esplits; eauto.
+          { rewrite list_fmap_insert //=. }
+          { rewrite list_fmap_insert //=. }
+          { eapply reqmap_rel_id; eauto. }
+          { intros i1; destruct (decide (i1 = stid)); subst; cycle 1.
+            { intros ???; rewrite list_lookup_insert_ne //=; apply Hlookup. }
+            { rewrite list_lookup_insert; ii; clarify.
+              split; ss. eapply (help_rel_call _ _ _ _ _ _ ctx rs (SchHdr.yield)); eauto.
+              { rewrite /HelpingOn.t /SchI.t; unseal CRIS; ss.
+                do 4 (apply elem_of_cons; right); apply elem_of_cons; left; ss.
+              }
+              intros ret; ss; eapply (help_rel_join _ _ ret _ _ n3); eauto.
+              { rewrite /join_pend /ccallU. grind. repeat f_equal; grind.
+                extensionalities a; destruct a; grind.
+              }
+              { rewrite /join_pend /ccallU. grind. repeat f_equal; grind.
+                extensionalities a; destruct a; grind.
+              }
+            }
+          }
+        }
+        (* join-None *)
+        rewrite ?interpV_ret; ired.
+        gstep; econs; eapply gsim_progress; try instantiate (1:=smj_bot); eauto using smj_le_bot.
+        gbase. eapply (CIH rs); eauto.
+        eexists (<[stid := (_, _, None)]> tl); esplits; eauto.
+        { rewrite list_fmap_insert //=. }
+        { rewrite list_fmap_insert //=. }
+        { eapply reqmap_rel_id; eauto. }
+        { intros i; destruct (decide (i = stid)); subst; cycle 1.
+          { intros ???; rewrite list_lookup_insert_ne //=; apply Hlookup. }
+          { rewrite list_lookup_insert; ii; clarify. }
+        }
       }
 
       destruct (decide (fn = SchHdr.yield)); subst.
-      { (* SchI.join *)
+      { (* SchI.yield *)
         rewrite {1 2}/LMod.prog ?alist_find_map_snd /=.
         destruct (dec _ _) as [?|e]; ss; [inv e; clear e|clarify; clear e].
         destruct (dec _ _) as [e|e]; ss; [inv e; clear e|clarify; clear e].
@@ -2218,21 +2205,405 @@ Section Helping.
         zprogress.
 
         rewrite /cfunU.
-        admit.
+        destruct (arg ↓) eqn : Harg; cycle 1.
+        { ss; iter_l; rewrite list_lookup_insert //= ?length_fmap //.
+          destruct (excluded_middle_informative _); step_l; ss.
+        }
+        ss. ired. rewrite /cgetU /=. ired.
+
+        replace_r; [rewrite interpV_bind interpV_vis //|]. ired.
+        eapply gsim_sGet_tgt;
+          [rewrite list_lookup_insert //= length_fmap //| ss | ].
+        esplits; eauto. rewrite list_insert_insert.
+
+        replace_l; [rewrite interpV_bind interpV_vis //|]. ired.
+        eapply gsim_sGet_src;
+          [rewrite list_lookup_insert //= length_fmap //| ss | ].
+        esplits; eauto. rewrite list_insert_insert.
+        rewrite ?interpV_ret. ired. hss. ired. rewrite ?interpV_ret. ired. hss. ired.
+
+        iter_l; rewrite list_lookup_insert //= ?length_fmap //. step_l; norm_l.
+        rewrite list_insert_insert.
+        iter_r; rewrite list_lookup_insert //= ?length_fmap //; step_r; norm_r.
+        rewrite list_insert_insert.
+
+        iter_l; rewrite list_lookup_insert //= ?length_fmap //. step_l; norm_l.
+        rewrite list_insert_insert.
+        iter_r; rewrite list_lookup_insert //= ?length_fmap //; step_r; norm_r.
+        rewrite list_insert_insert. ired.
+
+        replace_r; [rewrite interpV_bind interpV_vis //|]. ired.
+        eapply gsim_sGet_tgt;
+          [rewrite list_lookup_insert //= length_fmap //| ss | ].
+        esplits; eauto. rewrite list_insert_insert.
+
+        replace_l; [rewrite interpV_bind interpV_vis //|]. ired.
+        eapply gsim_sGet_src;
+          [rewrite list_lookup_insert //= length_fmap //| ss | ].
+        esplits; eauto. rewrite list_insert_insert.
+        rewrite ?interpV_ret. ired. hss. ired. rewrite ?interpV_ret. ired. hss. ired.
+
+        destruct (ths !! mtid) as [[smtid reto_s]|] eqn : Hmtid; cycle 1.
+        { rewrite Hmtid /=.
+          ss; iter_l; rewrite list_lookup_insert //= ?length_fmap //.
+          destruct (excluded_middle_informative _); step_l; ss.
+        }
+        rewrite Hmtid //=.
+        destruct (decide (smtid = stid)); subst; cycle 1.
+        { ss; iter_l; rewrite list_lookup_insert //= ?length_fmap //.
+          destruct (excluded_middle_informative _); step_l; ss.
+        }
+
+        ired.
+
+        replace_r; [rewrite interpV_bind interpV_trigger //=|]; ired.
+        eapply gsim_Choose_tgt; [rewrite list_lookup_insert // length_fmap //|].
+        intros [[mtidn stidn] Hmtidn]; rewrite list_insert_insert; ired; ss.
+
+        replace_l; [rewrite interpV_bind interpV_trigger //=|]; ired.
+        eapply gsim_Choose_src; [rewrite list_lookup_insert // length_fmap //|].
+        unshelve eexists (exist _ (mtidn, stidn) _); ss; eauto.
+        rewrite list_insert_insert; ired; ss.
+
+        ired. replace_r; [rewrite interpV_bind //|]. ired.
+        eapply gsim_s_cput_tgt; [rewrite list_lookup_insert // length_fmap //| |]; s.
+        { rewrite String.eqb_refl //. }
+        rewrite ?list_insert_insert.
+        rewrite /alist_upd /=; destruct (dec _ _) as [e|e]; ss; clarify; clear e.
+
+        ired. replace_l; [rewrite interpV_bind //|]. ired.
+        eapply gsim_s_cput_src; [rewrite list_lookup_insert // length_fmap //| |]; s.
+        { rewrite String.eqb_refl //. }
+        rewrite ?list_insert_insert.
+        rewrite /alist_upd /=; destruct (dec _ _) as [e|e]; ss; clarify; clear e.
+
+        iter_l; rewrite list_lookup_insert //= ?length_fmap //. step_l; norm_l.
+        rewrite list_insert_insert. hss.
+        iter_l; rewrite list_lookup_insert //= ?length_fmap //. step_l; norm_l.
+        rewrite list_insert_insert. hss. ired. rewrite ?interpV_ret. ired.
+
+        iter_r; rewrite list_lookup_insert //= ?length_fmap //. step_r; norm_r.
+        rewrite list_insert_insert. hss.
+        iter_r; rewrite list_lookup_insert //= ?length_fmap //. step_r; norm_r.
+        rewrite list_insert_insert. hss. ired. rewrite ?interpV_ret. ired.
+
+        gstep; econs; eapply gsim_progress; try instantiate (1:=smj_bot); eauto using smj_le_bot.
+        gbase. eapply (CIH rs); eauto.
+        eexists (<[stid := (_, _, None)]> tl); esplits; eauto.
+        { rewrite list_fmap_insert //=. }
+        { rewrite list_fmap_insert //=. }
+        { eapply reqmap_rel_id; eauto. }
+        { intros i; destruct (decide (i = stid)); subst; cycle 1.
+          { intros ???; rewrite list_lookup_insert_ne //=; apply Hlookup. }
+          { rewrite list_lookup_insert; ii; clarify. }
+        }
       }
-      admit.
+
+      destruct (decide (fn = SchHdr.get_tid)); subst.
+      { (* SchI.get_tid *)
+        rewrite {1 2}/LMod.prog ?alist_find_map_snd /=.
+        destruct (dec _ _) as [?|e]; ss; [inv e; clear e|clarify; clear e].
+        destruct (dec _ _) as [e|e]; ss; [inv e; clear e|clarify; clear e].
+        i; clarify.
+
+        revert Htid; unfold_trans; rewrite /SModTr.trans /SchI.get_tid.
+        intros Hstid.
+
+        eapply gsim_tau_src; [rewrite list_lookup_fmap // Hstid //=|].
+        eapply gsim_tau_tgt; [rewrite list_lookup_fmap // Hstid //=|].
+        zprogress.
+
+        rewrite /cfunU.
+        destruct (arg ↓) eqn : Harg; cycle 1.
+        { ss; iter_l; rewrite list_lookup_insert //= ?length_fmap //.
+          destruct (excluded_middle_informative _); step_l; ss.
+        }
+        ss. ired. rewrite /cgetU /=. ired.
+
+        replace_r; [rewrite interpV_bind interpV_vis //|]. ired.
+        eapply gsim_sGet_tgt;
+          [rewrite list_lookup_insert //= length_fmap //| ss | ].
+        esplits; eauto. rewrite list_insert_insert.
+
+        replace_l; [rewrite interpV_bind interpV_vis //|]. ired.
+        eapply gsim_sGet_src;
+          [rewrite list_lookup_insert //= length_fmap //| ss | ].
+        esplits; eauto. rewrite list_insert_insert.
+        rewrite ?interpV_ret. ired. hss. ired. rewrite ?interpV_ret. ired. hss. ired.
+        rewrite ?interpV_ret; ired.
+
+        gstep; econs; eapply gsim_progress; try instantiate (1:=smj_bot); eauto using smj_le_bot.
+        gbase. eapply (CIH rs); eauto.
+        eexists (<[stid := (_, _, None)]> tl); esplits; eauto.
+        { rewrite list_fmap_insert //=. }
+        { rewrite list_fmap_insert //=. }
+        { eapply reqmap_rel_id; eauto. }
+        { intros i; destruct (decide (i = stid)); subst; cycle 1.
+          { intros ???; rewrite list_lookup_insert_ne //=; apply Hlookup. }
+          { rewrite list_lookup_insert; ii; clarify. }
+        }
+      }
+
+      exfalso; revert H2; rewrite /HelpingOn.t /SchI.t; unseal CRIS; ss.
+      set_solver.
+    }
+
+    { (* inner spawn - continuation *)
+      rewrite /inner_spawn_pend in Htid.
+      iter_l; rewrite list_lookup_fmap Htid /=. step_l; norm_l.
+      iter_r; rewrite list_lookup_fmap Htid /=. step_r; norm_r.
+
+      destruct (arg ↓) eqn : Harg; ss; cycle 1.
+      { ired; replace_l; [rewrite interpV_bind interpV_trigger //|]. ired.
+        eapply gsim_Take_src; [rewrite list_lookup_insert // length_fmap //|]. ss.
+      }
+
+      ired.
+      replace_r; [rewrite interpV_bind //|]. ired.
+      eapply gsim_s_cgetU_tgt; [rewrite list_lookup_insert // length_fmap //| |]; s.
+      { rewrite String.eqb_refl //. }
+      esplits; eauto.
+      rewrite ?list_insert_insert. ired.
+
+      ired.
+      replace_r; [rewrite interpV_bind //|]. ired.
+      eapply gsim_s_cgetU_tgt; [rewrite list_lookup_insert // length_fmap //| |]; s.
+      { rewrite String.eqb_refl //. }
+      esplits; eauto.
+      rewrite ?list_insert_insert. ired.
+
+      ired.
+      replace_l; [rewrite interpV_bind //|]. ired.
+      eapply gsim_s_cgetU_src; [rewrite list_lookup_insert // length_fmap //| |]; s.
+      { rewrite String.eqb_refl //. }
+      esplits; eauto.
+      rewrite ?list_insert_insert. ired.
+
+      ired.
+      replace_l; [rewrite interpV_bind //|]. ired.
+      eapply gsim_s_cgetU_src; [rewrite list_lookup_insert // length_fmap //| |]; s.
+      { rewrite String.eqb_refl //. }
+      esplits; eauto.
+      rewrite ?list_insert_insert. ired.
+
+      des_ifs; cycle 1.
+      { ired; replace_l; [rewrite interpV_bind interpV_trigger //|]. ired.
+        eapply gsim_Take_src; [rewrite list_lookup_insert // length_fmap //|]. ss.
+      }
+
+      ired.
+      replace_r; [rewrite interpV_bind //|]. ired.
+      eapply gsim_s_cput_tgt; [rewrite list_lookup_insert // length_fmap //| |]; s.
+      { rewrite String.eqb_refl //. }
+      rewrite ?list_insert_insert. ired.
+
+      ired.
+      replace_l; [rewrite interpV_bind //|]. ired.
+      eapply gsim_s_cput_src; [rewrite list_lookup_insert // length_fmap //| |]; s.
+      { rewrite String.eqb_refl //. }
+      rewrite ?list_insert_insert. ired.
+
+      gstep; econs; eapply gsim_progress; try instantiate (1:=smj_bot); eauto using smj_le_bot.
+      gbase. eapply (CIH rs); eauto.
+      eexists (<[stid := (_, _, None)]> tl); esplits; eauto.
+      { rewrite list_fmap_insert //=. }
+      { rewrite list_fmap_insert //=. }
+      { eapply reqmap_rel_id; eauto. }
+      { intros stid2; destruct (decide (stid2 = stid)); subst; cycle 1.
+        { intros itr_s2 itr_t2 no2; rewrite list_lookup_insert_ne //=.
+          intros Hi; pose proof Hi as Hi'; revert Hi'; intros [Hi1 Hi2]%Hlookup; split; eauto.
+          destruct no2 as [[tid2 [b2 jid2]]|]; ss.
+          destruct Hi2 as [mtid2 [ro2 Hi2]]; apply lookup_lt_Some in Hi2 as Hlen2.
+          destruct (decide (mtid2 = mtid)); subst.
+          { rewrite Hi2 in Heq; clarify. exists mtid, (Some t); rewrite list_lookup_insert //. }
+          exists mtid2, ro2; rewrite list_lookup_insert_ne //.
+        }
+        { rewrite list_lookup_insert; ii; clarify. split; ss.
+          eapply help_rel_terminate; eauto.
+        }
+      }
+    }
+
+    { (* join - continuation*)
+      rewrite /join_pend in Htid.
+      iter_l; rewrite list_lookup_fmap Htid /=. step_l; norm_l.
+      iter_r; rewrite list_lookup_fmap Htid /=. step_r; norm_r.
+
+      destruct (arg ↓) eqn : Harg; ss; cycle 1.
+      { ired; replace_l; [rewrite interpV_bind interpV_trigger //|]. ired.
+        eapply gsim_Take_src; [rewrite list_lookup_insert // length_fmap //|]. ss.
+      }
+
+      ired.
+      rewrite unfold_iterC; ired.
+      rewrite {1 2}interpV_tau.
+      eapply gsim_tau_src; [rewrite list_lookup_insert // length_fmap //|].
+      eapply gsim_tau_tgt; [rewrite list_lookup_insert // length_fmap //|].
+      rewrite !list_insert_insert.
+
+      replace_l; [rewrite interpV_bind //|]. ired.
+      eapply gsim_s_cgetU_src; [rewrite list_lookup_insert // length_fmap //| |]; s.
+      { rewrite String.eqb_refl //. }
+      esplits; eauto.
+      rewrite ?list_insert_insert. ired.
+
+      replace_r; [rewrite interpV_bind //|]. ired.
+      eapply gsim_s_cgetU_tgt; [rewrite list_lookup_insert // length_fmap //| |]; s.
+      { rewrite String.eqb_refl //. }
+      esplits; eauto.
+      rewrite ?list_insert_insert. ired.
+
+      destruct (ths !! tid) as [[? [rv|]]|] eqn : Hret; rewrite Hret /=; ired.
+      { (* Join-return *)
+        rewrite ?interpV_ret; ired.
+        gstep; econs; eapply gsim_progress; try instantiate (1:=smj_bot); eauto using smj_le_bot.
+        gbase. eapply (CIH rs); eauto.
+        eexists (<[stid := (_, _, None)]> tl); esplits; eauto.
+        { rewrite list_fmap_insert //=. }
+        { rewrite list_fmap_insert //=. }
+        { eapply reqmap_rel_id; eauto. }
+        { intros i; destruct (decide (i = stid)); subst; cycle 1.
+          { intros ???; rewrite list_lookup_insert_ne //=; apply Hlookup. }
+          { rewrite list_lookup_insert; ii; clarify. }
+        }
+      }
+      { (* Join-loop *)
+        rewrite /ccallU.
+
+        iter_l. rewrite list_lookup_insert /=; [|rewrite length_fmap //]. step_l. norm_l.
+        rewrite list_insert_insert.
+        iter_r. rewrite list_lookup_insert /=; [|rewrite length_fmap //]. step_r. norm_r.
+        rewrite list_insert_insert. ired.
+
+        destruct ((wmask_and msk wmask_all) SchHdr.yield) eqn : Hfn; cycle 1.
+        { iter_l; rewrite list_lookup_insert /=; [rewrite Hfn /=|rewrite length_fmap //].
+          step_l; ss.
+        }
+
+        iter_l; rewrite ?list_lookup_insert /=; last rewrite ?length_fmap //. rewrite Hfn /=.
+        iter_r; rewrite ?list_lookup_insert /=; last rewrite ?length_fmap //. rewrite Hfn /=.
+        step_l; step_r. norm_l; norm_r.
+        destruct (prog_s ctx rs SchHdr.yield) eqn : Hfn_s; cycle 1.
+        { step_l; ss. }
+        destruct (prog_t ctx rs SchHdr.yield) eqn : Hfn_t; cycle 1.
+        { eapply prog_s_prog_t in Hfn_s as Hfn_t'; des; clarify. }
+        norm_l; norm_r.
+        rewrite !list_insert_insert. ired.
+        gstep; econs; eapply gsim_progress; try instantiate (1:=smj_bot); eauto using smj_le_bot.
+        gbase. eapply (CIH rs); eauto.
+        eexists (<[stid := (_, _, None)]> tl); esplits; eauto.
+        { rewrite list_fmap_insert //=. }
+        { rewrite list_fmap_insert //=. }
+        { eapply reqmap_rel_id; eauto. }
+        { intros i1; destruct (decide (i1 = stid)); subst; cycle 1.
+          { intros ???; rewrite list_lookup_insert_ne //=; apply Hlookup. }
+          { rewrite list_lookup_insert; ii; clarify.
+            split; ss. eapply (help_rel_call _ _ _ _ _ _ ctx rs (SchHdr.yield)); eauto.
+            { rewrite /HelpingOn.t /SchI.t; unseal CRIS; ss.
+              do 4 (apply elem_of_cons; right); apply elem_of_cons; left; ss.
+            }
+            intros ret; ss; eapply (help_rel_join _ _ ret _ _ tid); eauto.
+            { rewrite /join_pend /ccallU. grind. repeat f_equal; grind.
+              extensionalities a; destruct a; grind.
+            }
+            { rewrite /join_pend /ccallU. grind. repeat f_equal; grind.
+              extensionalities a; destruct a; grind.
+            }
+          }
+        }
+      }
+      (* join-None *)
+      rewrite ?interpV_ret; ired.
+      gstep; econs; eapply gsim_progress; try instantiate (1:=smj_bot); eauto using smj_le_bot.
+      gbase. eapply (CIH rs); eauto.
+      eexists (<[stid := (_, _, None)]> tl); esplits; eauto.
+      { rewrite list_fmap_insert //=. }
+      { rewrite list_fmap_insert //=. }
+      { eapply reqmap_rel_id; eauto. }
+      { intros i; destruct (decide (i = stid)); subst; cycle 1.
+        { intros ???; rewrite list_lookup_insert_ne //=; apply Hlookup. }
+        { rewrite list_lookup_insert; ii; clarify. }
+      }
+    }
+
+    { (* inner_spawn - continuation*)
+      revert Htid; rewrite /Sch.terminate; unseal SCH; rewrite unfold_iterC. ired.
+      rewrite {1 2}interpV_tau; intros Htid.
+      eapply gsim_tau_src; [rewrite list_lookup_fmap Htid //|].
+      eapply gsim_tau_tgt; [rewrite list_lookup_fmap Htid //|].
+
+      iter_l. rewrite list_lookup_insert /=; [|rewrite length_fmap //]. step_l. norm_l.
+      rewrite list_insert_insert.
+      iter_r. rewrite list_lookup_insert /=; [|rewrite length_fmap //]. step_r. norm_r.
+      rewrite list_insert_insert. ired.
+
+      destruct ((wmask_and msk wmask_all) SchHdr.yield) eqn : Hfn; cycle 1.
+      { iter_l; rewrite list_lookup_insert /=; [rewrite Hfn /=|rewrite length_fmap //].
+        step_l; ss.
+      }
+
+      iter_l; rewrite ?list_lookup_insert /=; last rewrite ?length_fmap //. rewrite Hfn /=.
+      iter_r; rewrite ?list_lookup_insert /=; last rewrite ?length_fmap //. rewrite Hfn /=.
+      step_l; step_r. norm_l; norm_r.
+      destruct (prog_s ctx rs SchHdr.yield) eqn : Hfn_s; cycle 1.
+      { step_l; ss. }
+      destruct (prog_t ctx rs SchHdr.yield) eqn : Hfn_t; cycle 1.
+      { eapply prog_s_prog_t in Hfn_s as Hfn_t'; des; clarify. }
+      norm_l; norm_r.
+      rewrite !list_insert_insert. ired.
+      gstep; econs; eapply gsim_progress; try instantiate (1:=smj_bot); eauto using smj_le_bot.
+      gbase. eapply (CIH rs); eauto.
+      eexists (<[stid := (_, _, None)]> tl); esplits; eauto.
+      { rewrite list_fmap_insert //=. }
+      { rewrite list_fmap_insert //=. }
+      { eapply reqmap_rel_id; eauto. }
+      { intros i1; destruct (decide (i1 = stid)); subst; cycle 1.
+        { intros ???; rewrite list_lookup_insert_ne //=; apply Hlookup. }
+        { rewrite list_lookup_insert; ii; clarify.
+          split; ss.
+          eapply (help_rel_call _ _ _ _ _ _ ctx rs (SchHdr.yield)); eauto.
+          { rewrite /HelpingOn.t /SchI.t; unseal CRIS; ss.
+            do 4 (apply elem_of_cons; right); apply elem_of_cons; left; ss.
+          }
+          i; ss.
+          eapply (help_rel_eq _ _ _ _ (tau;; Ret ret)).
+          { unfold_trans; rewrite ?interpV_tau ?interpV_ret.
+            instantiate (1:= λ x : Any.t,
+              x <- ⇓cris (⇓sb(false, wmask_and msk wmask_all, SchI.scopes) (⇓smod(false, sp_none)
+                (x <- Sch.terminate;; Ret x↑)));;
+              ktr_t x).
+            rewrite /Sch.terminate; unseal SCH. grind.
+          }
+          { unfold_trans; rewrite ?interpV_tau ?interpV_ret.
+            instantiate (1:= λ x : Any.t,
+              x <- ⇓cris (⇓sb(false, wmask_and msk wmask_all, SchI.scopes) (⇓smod(false, sp_none)
+                (x <- Sch.terminate;; Ret x↑)));;
+              ktr_s x).
+            rewrite /Sch.terminate; unseal SCH. grind.
+          }
+          { instantiate (1:=[]); set_solver. }
+          { ii; clarify. }
+          i; ss.
+          eapply help_rel_terminate; eauto.
+        }
+      }
+    }
+
+    { (* Return case *)
+      iter_l; iter_r; rewrite ?list_lookup_fmap Htid /=.
+      step_l; step_r; norm_l; norm_r.
+      des_ifs; ss.
+      { rewrite /LModTr.interp_stateE ?interp_state_ret; ired.
+        gstep; econs; econs; ss.
+      }
+      rewrite /triggerUB; ss; step_l; ss.
     }
 
     rename itr into itr_c.
     rename H4 into Hscp.
     destruct (case_itrH itr_c) as [[v ->]|Hf].
     { (* return case *)
-      iter_l; iter_r; rewrite ?list_lookup_fmap Htid /=.
-      norm_l. step_l. norm_r. step_r.
-      des_ifs; ss; cycle 1.
-      { norm_l. step_l. ss. }
-      norm_l. norm_r.
-      zstep; rewrite /HelpingOff.t /HelpingOn.t /SchI.t; unseal CRIS; ss.
+      exfalso; eapply H5; eauto.
     }
     destruct Hf as [[f' ->]|Hf].
     { (* tau case *)
@@ -2247,17 +2618,18 @@ Section Helping.
       { intros i; destruct (decide (i = stid)); subst; cycle 1.
         { intros ???; rewrite list_lookup_insert_ne //=; apply Hlookup. }
         { rewrite list_lookup_insert; ii; clarify. split; ss.
-          eapply help_rel_eq; eauto. rewrite bind_ret_r //.
+          ides f'.
+          { rewrite ?interpV_ret; ired; eauto. }
+          { eapply help_rel_eq; eauto. }
+          { eapply help_rel_eq; eauto. }
         }
       }
     }
     destruct Hf as [[P [f' ->]]|Hf].
     { (* Assume *)
       eapply gsim_Assume_src; [rewrite list_lookup_fmap Htid //=|].
-      { grind. }
       intros r_s2 -> Hr_s2.
       eapply gsim_Assume_tgt; [rewrite list_lookup_fmap Htid //=|].
-      { grind. }
       exists r_s2; esplits; try by des.
       gstep; econs; eapply gsim_progress; try instantiate (1:=smj_bot); eauto using smj_le_bot.
       gbase. eapply (CIH r_s2); try by des.
@@ -2268,17 +2640,20 @@ Section Helping.
       { intros i; destruct (decide (i = stid)); subst; cycle 1.
         { intros ???; rewrite list_lookup_insert_ne //=; apply Hlookup. }
         { rewrite list_lookup_insert; ii; clarify. split; ss.
-          eapply help_rel_eq; eauto. rewrite bind_ret_r //.
+          ides f'.
+          { rewrite ?interpV_ret; ired; eauto. }
+          { eapply help_rel_eq; eauto. }
+          { eapply help_rel_eq; eauto. }
         }
       }
     }
     destruct Hf as [[res [f' ->]]|Hf].
     { (* AssumeRes *)
       eapply gsim_AssumeRes_src; [rewrite list_lookup_fmap Htid //=|].
-      { f_equal. grind. repeat f_equal; extensionalities a; destruct a; ss. }
+      { unfold_trans. instantiate (1:=k_s). repeat f_equal. extensionalities a; destruct a; ss. }
       intros Hval.
       eapply gsim_AssumeRes_tgt; [rewrite list_lookup_fmap Htid //=|].
-      { f_equal; grind. repeat f_equal. extensionalities a; destruct a; ss. }
+      { unfold_trans. instantiate (1:=k_t). repeat f_equal. extensionalities a; destruct a; ss. }
       split; first done.
 
       gstep; econs; eapply gsim_progress; try instantiate (1:=smj_bot); eauto using smj_le_bot.
@@ -2290,17 +2665,18 @@ Section Helping.
       { intros i; destruct (decide (i = stid)); subst; cycle 1.
         { intros ???; rewrite list_lookup_insert_ne //=; apply Hlookup. }
         { rewrite list_lookup_insert; ii; clarify. split; ss.
-          eapply help_rel_eq; eauto. rewrite bind_ret_r //.
+          ides (f' ()).
+          { rewrite ?interpV_ret; ired; eauto. }
+          { eapply help_rel_eq; eauto. }
+          { eapply help_rel_eq; eauto. }
         }
       }
     }
     destruct Hf as [[P [f' ->]]|Hf].
     { (* Guarantee *)
       eapply gsim_Guarantee_tgt; [rewrite list_lookup_fmap Htid //=|].
-      { f_equal. grind. }
       intros r2 ?.
       eapply gsim_Guarantee_src; [rewrite list_lookup_fmap Htid //=|].
-      { f_equal; grind. }
       esplits; try by des.
 
       gstep; econs; eapply gsim_progress; try instantiate (1:=smj_bot); eauto using smj_le_bot.
@@ -2312,7 +2688,10 @@ Section Helping.
       { intros i; destruct (decide (i = stid)); subst; cycle 1.
         { intros ???; rewrite list_lookup_insert_ne //=; apply Hlookup. }
         { rewrite list_lookup_insert; ii; clarify. split; ss.
-          eapply help_rel_eq; eauto. rewrite bind_ret_r //.
+          ides (f').
+          { rewrite ?interpV_ret; ired; eauto. }
+          { eapply help_rel_eq; eauto. }
+          { eapply help_rel_eq; eauto. }
         }
       }
     }
@@ -2341,12 +2720,37 @@ Section Helping.
       { intros i; destruct (decide (i = stid)); subst; cycle 1.
         { intros ???; rewrite list_lookup_insert_ne //=; apply Hlookup. }
         { rewrite list_lookup_insert; ii; clarify. split; ss.
-          eapply help_rel_call; eauto.
-          intros ret; eapply help_rel_eq; eauto.
-          ired. unfold_trans. instantiate (1:=tau;; k ret).
-          rewrite ?interpV_tau //.
+          destruct (decide (Some fn ∈
+            List.map fst (Mod.fnsems ((HelpingOn.t mn jobs sp) ★ (CFilter.filter msk SchI.t))))).
+          { eapply (help_rel_call _ _ _ _ _ _ ctx); eauto. intros ret; ss.
+            eapply (help_rel_eq _ _ k_s k_t (tau;; k ret)); eauto.
+            { grind. unfold_trans. rewrite ?interpV_tau; grind. }
+            { grind. unfold_trans. rewrite ?interpV_tau; grind. }
+          }
+          hexploit (prog_fn_ctx fn ctx rs); eauto.
+          intros [Hs|[itr_ctx [img1 [msk1 [scp1 [Ht [Hs ?]]]]]]]; clarify.
+          rewrite Ht Hs in H_prog_t'; inv H_prog_t'.
+          ides (itr_ctx args).
+          { rewrite ?interpV_ret; ired.
+            eapply (help_rel_eq _ _ k_s k_t (tau;; k r0) img_c msk_c scp_c); eauto.
+            { unfold_trans. rewrite ?interpV_tau; grind. }
+            { unfold_trans. rewrite ?interpV_tau; grind. }
+          }
+          { eapply (help_rel_eq _ _ _ _ (tau;; t)); eauto.
+            ii; ss.
+            eapply (help_rel_eq _ _ k_s k_t (tau;; k ret) img_c msk_c scp_c); eauto.
+            { unfold_trans. rewrite ?interpV_tau; grind. }
+            { unfold_trans. rewrite ?interpV_tau; grind. }
+          }
+          { eapply (help_rel_eq _ _ _ _ (Vis e k0)); eauto.
+            ii; ss.
+            eapply (help_rel_eq _ _ k_s k_t (tau;; k ret) img_c msk_c scp_c); eauto.
+            { unfold_trans. rewrite ?interpV_tau; grind. }
+            { unfold_trans. rewrite ?interpV_tau; grind. }
+          }
         }
       }
+      eauto.
     }
     { (* Spawn case *)
       rename img into img_c, msk0 into msk_c, scp into scp_c.
@@ -2368,29 +2772,52 @@ Section Helping.
       { rewrite ?fmap_app list_fmap_insert //=. }
       { rewrite ?fmap_app list_fmap_insert //=. }
       { eapply reqmap_rel_append; eauto.
-        eapply reqmap_rel_id; eauto.  
+        eapply reqmap_rel_id; eauto.
       }
       { intros i; destruct (decide (i = length tl)); subst.
         { intros ???; rewrite lookup_app_r // ?length_insert; try lia.
           rewrite Nat.sub_diag /=; intros Heq; inv Heq.
           split; ss.
-          eapply help_rel_call; eauto.
-          { instantiate (1:=λ a, Ret a); ired; refl. }
-          { instantiate (1:=λ a, Ret a); ired; refl. }
-          intros res; eapply help_rel_eq; eauto.
-          instantiate (1:=Ret res); unfold_trans; rewrite ?interpV_ret //.
+          destruct (decide (Some fn ∈
+            List.map fst (Mod.fnsems ((HelpingOn.t mn jobs sp) ★ (CFilter.filter msk SchI.t))))).
+          { eapply (help_rel_call _ _ _ _ (λ a, Ret a) (λ a, Ret a) ctx); eauto.
+            { grind. }
+            { grind. }
+            intros ret; ss. apply help_rel_ret.
+          }
+          hexploit (prog_fn_ctx fn ctx rs); eauto.
+          intros [Hs|[itr_ctx [img1 [msk1 [scp1 [Ht [Hs ?]]]]]]]; clarify.
+          rewrite Ht Hs in H_prog_t'; inv H_prog_t'.
+          ides (itr_ctx args).
+          { rewrite ?interpV_ret; ired.
+            apply help_rel_ret.
+          }
+          { eapply (help_rel_eq _ _ (λ a, Ret a) (λ a, Ret a) (tau;; t)); eauto.
+            { grind. }
+            { grind. }
+            ii; apply help_rel_ret.
+          }
+          { eapply (help_rel_eq _ _ (λ a, Ret a) (λ a, Ret a) (Vis e k0)); eauto.
+            { grind. }
+            { grind. }
+            ii; apply help_rel_ret.
+          }
         }
         destruct (decide (i = stid)); subst.
         { intros ???; rewrite -insert_app_l // list_lookup_insert // ?length_app; try lia.
           intros EQ; clarify.
           split; ss.
-          eapply help_rel_eq; eauto.
-          rewrite ?length_fmap //.
+          rewrite ?length_fmap.
+          ides (k (length tl)).
+          { rewrite ?interpV_ret; ired. eauto. }
+          { eapply (help_rel_eq _ _ k_s k_t (tau;; t)); eauto. }
+          { eapply (help_rel_eq _ _ k_s k_t (Vis e k0)); eauto. }
         }
         rewrite -insert_app_l // list_lookup_insert_ne //.
         intros ??? [[Hilen Hi]|[??]]%lookup_snoc_Some; last clarify.
         apply Hlookup; eauto.
       }
+      eauto.
     }
 
     { (* Yield case *)
@@ -2404,8 +2831,11 @@ Section Helping.
       { eapply reqmap_rel_id; eauto. }
       { intros i; destruct (decide (i = stid)); subst; cycle 1.
         { intros ???; rewrite list_lookup_insert_ne //=; apply Hlookup. }
-        { rewrite list_lookup_insert; ii; clarify. split; ss.
-          eapply help_rel_eq; eauto. ired; refl.
+        { rewrite list_lookup_insert; ii; clarify. ired. split; ss.
+          ides (k ()).
+          { rewrite ?interpV_ret; ired; eauto. }
+          { eapply (help_rel_eq _ _ k_s k_t (tau;; t)); eauto. }
+          { eapply (help_rel_eq _ _ k_s k_t (Vis e k0)); eauto. }
         }
       }
     }
@@ -2421,8 +2851,11 @@ Section Helping.
       { eapply reqmap_rel_id; eauto. }
       { intros i; destruct (decide (i = stid)); subst; cycle 1.
         { intros ???; rewrite list_lookup_insert_ne //=; apply Hlookup. }
-        { rewrite list_lookup_insert; ii; clarify. split; ss.
-          eapply help_rel_eq; eauto. ired; refl.
+        { rewrite list_lookup_insert; ii; clarify. split; ss. ired.
+          ides (k stid).
+          { rewrite ?interpV_ret; ired; eauto. }
+          { eapply (help_rel_eq _ _ k_s k_t (tau;; t)); eauto. }
+          { eapply (help_rel_eq _ _ k_s k_t (Vis e k0)); eauto. }
         }
       }
     }
@@ -2467,8 +2900,11 @@ Section Helping.
         { eapply reqmap_rel_id; eauto. }
         { intros i; destruct (decide (i = stid)); subst; cycle 1.
           { intros ???; rewrite list_lookup_insert_ne //=; apply Hlookup. }
-          { rewrite list_lookup_insert; ii; clarify. split; ss.
-            eapply help_rel_eq; eauto.
+          { rewrite list_lookup_insert; ii; clarify. split; ss. ired.
+            ides (f' ()).
+            { rewrite ?interpV_ret; ired; eauto. }
+            { eapply (help_rel_eq _ _ k_s k_t (tau;; t)); eauto. }
+            { eapply (help_rel_eq _ _ k_s k_t (Vis e k0)); eauto. }
           }
         }
       }
@@ -2507,8 +2943,11 @@ Section Helping.
         { eapply reqmap_rel_id; eauto. }
         { intros i; destruct (decide (i = stid)); subst; cycle 1.
           { intros ???; rewrite list_lookup_insert_ne //=; apply Hlookup. }
-          { rewrite list_lookup_insert; ii; clarify. split; ss.
-            eapply help_rel_eq; eauto.
+          { rewrite list_lookup_insert; ii; clarify. split; ss. ired.
+            ides (f' (or_else (alist_find k st_ctx) ()↑)).
+            { rewrite ?interpV_ret; ired; eauto. }
+            { eapply (help_rel_eq _ _ k_s k_t (tau;; t)); eauto. }
+            { eapply (help_rel_eq _ _ k_s k_t (Vis e k0)); eauto. }
           }
         }
       }
@@ -2531,8 +2970,11 @@ Section Helping.
       { eapply reqmap_rel_id; eauto. }
       { intros i; destruct (decide (i = stid)); subst; cycle 1.
         { intros ???; rewrite list_lookup_insert_ne //=; apply Hlookup. }
-        { rewrite list_lookup_insert; ii; clarify. split; ss.
-          eapply help_rel_eq; eauto. ired; refl.
+        { rewrite list_lookup_insert; ii; clarify. split; ss. ired.
+          ides (f' x).
+          { rewrite ?interpV_ret; ired; eauto. }
+          { eapply (help_rel_eq _ _ k_s k_t (tau;; t)); eauto. }
+          { eapply (help_rel_eq _ _ k_s k_t (Vis e k)); eauto. }
         }
       }
     }
@@ -2552,8 +2994,11 @@ Section Helping.
       { eapply reqmap_rel_id; eauto. }
       { intros i; destruct (decide (i = stid)); subst; cycle 1.
         { intros ???; rewrite list_lookup_insert_ne //=; apply Hlookup. }
-        { rewrite list_lookup_insert; ii; clarify. split; ss.
-          eapply help_rel_eq; eauto. ired; refl.
+        { rewrite list_lookup_insert; ii; clarify. split; ss. ired.
+          ides (f' x).
+          { rewrite ?interpV_ret; ired; eauto. }
+          { eapply (help_rel_eq _ _ k_s k_t (tau;; t)); eauto. }
+          { eapply (help_rel_eq _ _ k_s k_t (Vis e k)); eauto. }
         }
       }
     }
@@ -2570,11 +3015,14 @@ Section Helping.
       { eapply reqmap_rel_id; eauto. }
       { intros i; destruct (decide (i = stid)); subst; cycle 1.
         { intros ???; rewrite list_lookup_insert_ne //=; apply Hlookup. }
-        { rewrite list_lookup_insert; ii; clarify. split; ss.
-          eapply help_rel_eq; eauto.
+        { rewrite list_lookup_insert; ii; clarify. split; ss. ired.
+          ides (f' x_tgt).
+          { rewrite ?interpV_ret; ired; eauto. }
+          { eapply (help_rel_eq _ _ k_s k_t (tau;; t)); eauto. }
+          { eapply (help_rel_eq _ _ k_s k_t (Vis e k)); eauto. }
         }
       }
     }
   Unshelve. all: eauto.
-  Admitted.
+  (*SLOW*)Admitted.
 End Helping.
