helping/HelpingFacts.v
@@ -1,97 +1,79 @@
-(* Require Import CRIS.
-Require Import SchHeader SchA.
+Require Import CRIS.
+Require Import SchHeader SchI.
 From CRIS.helping Require Import Header HelpingOn HelpingOff HelpingOnOffproof.
 
 Section Helping.
-  Context `{!crisG Γ Σ α β τ _S _I, !schG}.
+  Context `{!crisG Γ Σ α β τ _S _I, !concG, !schG}.
 
   (* Lemmas about names *)
-  Definition strings_maxlen (l: list string) : nat :=
+  Definition strings_maxlen (l : list string) : nat :=
     list_max (List.map String.length l).
 
-  Fixpoint mname_long (n: nat) : string :=
+  Fixpoint mname_long (n : nat) : string :=
     match n with
     | 0 => ""
     | S n' => "h" +:+ mname_long n'
     end.
 
-  Lemma mname_long_length n:
+  Lemma mname_long_length n :
     String.length (mname_long n) = n.
   Proof.
     induction n; ss.
     rewrite IHn. et.
   Qed.
 
-  Lemma strings_maxlen_app l1 l2:
-    strings_maxlen (l1++l2) = max (strings_maxlen l1) (strings_maxlen l2).
+  Lemma strings_maxlen_app l1 l2 :
+    strings_maxlen (l1 ++ l2) = max (strings_maxlen l1) (strings_maxlen l2).
   Proof.
     revert l2. induction l1; et.
     i. s. unfold strings_maxlen in *. ss.
     rewrite IHl1. nia.
   Qed.
 
-  Lemma long_name_notin l (fn: string)
-    (LONG: String.length fn > strings_maxlen l)
-    :
+  Lemma long_name_notin l (fn : string) :
+    String.length fn > strings_maxlen l →
     ~ wmask_list l fn.
   Proof.
-    ii. eapply existsb_exists in H0. des. eapply String.eqb_eq in H1; subst.
+    intros Hlen Hmsk. eapply existsb_exists in Hmsk. des. eapply String.eqb_eq in Hmsk0; subst.
     revert_until l. induction l; i; ss.
     des; subst.
-    - rewrite /strings_maxlen in LONG. ss. nia.
+    - rewrite /strings_maxlen in Hlen. ss. nia.
     - eapply IHl; et. unfold strings_maxlen in *. ss. nia.
   Qed.
 
-  (* Lemma sch_pure_elim_filter msk u sp_s:
+  Lemma helping_on_wf jobID (jobs : jobID -> _) mn sp : Mod.wf (HelpingOn.t mn jobs sp).
+  Proof. unfold_mod. econs; ss; prove_nodup. Qed.
+
+  (* imp : list of function names mI calls *)
+  Theorem helping_main (mA mM mI : Mod.t) (P1 P2 : iProp Σ) imp jobID (jobs : jobID -> _) sp :
+    (∀ mn msk,
+      ((Helping.exports mn) ## imp →
+      wmask_sub (wmask_list imp) msk →
+      ctx_refines
+        (mM ★ (HelpingOn.t mn jobs sp) ★ CFilter.filter msk SchI.t, P1)
+        (CFilter.filter msk mI ★ CFilter.filter msk SchI.t, emp%I))) →
+    (∀ mn msk,
+      ((Helping.exports mn) ## imp →
+      wmask_sub (wmask_list imp) msk →
+      ctx_refines
+        (mA ★ CFilter.filter msk SchI.t, P2)
+        (mM ★ HelpingOff.t mn jobs sp ★ CFilter.filter msk SchI.t, emp%I))) →
     ctx_refines
-      (SchAPure.t u sp_s, emp%I)
-      (CFilter.filter msk (SchAPure.t u sp_s), emp%I).
+      (mA ★ SchI.t, (P1 ∗ P2)%I)
+      (mI ★ SchI.t, emp%I).
   Proof.
-    eapply main_adequacy with (Ist := fun _ _ _ => emp%I).
-    init_sim; et.
-    init_simF u u.
-
-    steps_l. forces_r. iSplitL "ASM"; et.
-    steps_r. forces_l. iSplitL "GRT"; et.
-    step; et.
-  Qed. *)
-
-  Lemma helping_on_wf jobID (jobs : jobID -> _) mn sp:
-    Mod.wf (HelpingOn.t mn jobs sp).
-  Proof. unfold_mod. econs; prove_nodup. Qed.
-
-  Theorem helping_main {mA mM mI P1 P2} imp jobID (jobs: jobID -> _) E q sp sp_s sp_u
-    (UserInSp: sp_incl sp_u sp_s)
-    (SchInSp : sp_incl (SchAS.sp sp_u E q) sp_s)
-    (MAIN  : ∀ mn msk
-                (DISJ: ∀ fn, In fn (Helping.exports mn) → In fn imp → False)
-                (SUB: wmask_sub (wmask_list imp) msk),
-        ctx_refines
-          (mM mn ★                 (HelpingOn.t mn jobs sp) ★ CFilter.filter msk (SchA.t sp_s sp_u), P1)
-          (CFilter.filter msk mI ★ (HelpingOn.t mn jobs sp) ★ CFilter.filter msk (SchA.t sp_s sp_u), emp%I))
-    (CANCEL: ∀ mn msk
-                (DISJ: ∀ fn, In fn (Helping.exports mn) → In fn imp → False)
-                (SUB: wmask_sub (wmask_list imp) msk),
-        ctx_refines
-          (mA                                ★ CFilter.filter msk (SchA.t sp_s sp_u), P2)
-          (mM mn ★ (HelpingOff.t mn jobs sp) ★ CFilter.filter msk (SchA.t sp_s sp_u), emp%I))
-    :
-    ctx_refines
-      (mA ★ (SchA.t sp_s sp_u), (P1 ∗ P2)%I)
-      (mI ★ (SchA.t sp_s sp_u), emp%I).
-  Proof.
-    intros [ctx P]; s.
+    intros Hc1 Hc2 [ctx P]; s.
     ctxr_norm.
 
     match goal with [|-refines (?src,?P1) (?tgt,?P2)] =>
       pose (md_src := src);
       pose (md_tgt := tgt);
       pose (all_names :=
-        imp ++ omap (id) (Mod.exports md_src) ++ omap (id) (Mod.exports md_tgt)
+        imp ++ omap id (Mod.exports md_src) ++ omap id (Mod.exports md_tgt)
                            ++ Mod.scopes md_src ++ Mod.scopes md_tgt);
       cut(List.NoDup (Mod.scopes tgt) -> refines (src,P1) (tgt,P2))
     end.
-    { ii. eapply H0; et. destruct WFM. et. }
+    { intros Hg WFM; ss. eapply Hg; et. destruct WFM. et. }
     intros NODUP.
 
     etrans; cycle 1.
@@ -102,32 +84,33 @@ Section Helping.
     pose (mn := mname_long (10 + strings_maxlen all_names)).
     pose (mask := wmask_list all_names).
 
-    (* assert (DISJ: ∀ fn, In fn (Helping.exports mn) → In fn imp → False).
-    { ii. eapply (long_name_notin _ fn); cycle 1.
-      * unfold wmask_list. eapply existsb_exists.
-        esplits; [apply H0|apply String.eqb_eq]; et.
-      * s in H0. des; ss; subst.
-        { subst mn. s.
+    assert (DISJ : Helping.exports mn ## imp).
+    { intros x H1 H2. eapply (long_name_notin _ x); cycle 1.
+      { unfold wmask_list. eapply existsb_exists.
+        esplits; [|apply String.eqb_eq]; et.
+        apply elem_of_list_In, H2.
+      }
+      { rewrite /Helping.exports elem_of_cons in H1. des; ss; subst.
+        { rewrite /Helping.exports /Helping.run /mn /=.
+          rewrite !strings_maxlen_app !string_length_app.
+          rewrite /Helping.exports mname_long_length /=. nia.
+        }
+        { apply elem_of_cons in H1; des; last inv H1. subst mn x. ss. fold append.
           rewrite !strings_maxlen_app !string_length_app.
           rewrite mname_long_length. nia.
         }
-        { subst mn. s. fold append.
-          rewrite !strings_maxlen_app !string_length_app.
-          rewrite mname_long_length. nia.
-        }
+      }
     }
 
-    assert(SUB: wmask_sub (wmask_list imp) mask).
-    {
-      unfold mask, wmask_sub, wmask_list.
-      i. eapply existsb_exists in H. des.
+    assert (SUB : wmask_sub (wmask_list imp) mask).
+    { unfold mask, wmask_sub, wmask_list.
+      intros ? Hin. eapply existsb_exists in Hin. des.
       eapply existsb_exists. esplits; et.
       eapply in_or_app; et.
-    } *)
+    }
 
     etrans; cycle 1.
-    { eapply CFilter.intro_module
-        with (mask:= mask) (mc := HelpingOn.t mn jobs sp); et.
+    { eapply CFilter.intro_module with (mask := mask) (mc := HelpingOn.t mn jobs sp); et.
       - eapply helping_on_wf.
       - i. r. rewrite existsb_exists.
         esplits; try apply String.eqb_eq; eauto.
@@ -135,26 +118,27 @@ Section Helping.
         eapply in_or_app; left; rewrite /Mod.exports; subst md_tgt.
         rewrite -elem_of_list_In elem_of_list_omap; eexists; rewrite elem_of_list_In //.
       - intros fn IN.
-        (* split; cycle 1. *)
-        (* { revert IN. unfold_hmod. s. i. des; subst; ss. } *)
         eapply long_name_notin.
-        revert IN. s. unfold_mod. s. i. des; subst; try by ss.
-        + inv IN. simpl String.length. fold append.
+        revert IN. unfold_mod. s. i. des; subst; try by ss.
+        { inv IN. simpl String.length. fold append.
           rewrite !strings_maxlen_app !string_length_app mname_long_length.
           nia.
-        + inv IN. simpl String.length. fold append.
+        }
+        { inv IN. simpl String.length. fold append.
           rewrite !strings_maxlen_app !string_length_app mname_long_length.
           nia.
-      - admit.
-      (* eapply List.NoDup_app; et.
-        + unfold_hmod. econs; ss. econs.
-        + ii. eapply (long_name_notin _ a); cycle 1.
-          * unfold wmask_list. eapply existsb_exists.
-            esplits; [apply H|apply String.eqb_eq]; et.
-          * revert H0; unfold_hmod. i. rr in H0. des; ss; subst.
-            unfold mn. rewrite !strings_maxlen_app. s.
-            rewrite mname_long_length. nia. *)
-          - admit.
+        }
+      - unfold_mod; ss; ii; des; ss.
+      - eapply List.NoDup_app.
+        + unfold_mod; ss.
+        + unfold_mod; ss. rewrite /HelpingOn.scopes; econs; ss. econs; ss.
+        + intros a Ha Ha2; eapply (long_name_notin _ a); cycle 1.
+          * rewrite /wmask_list; eapply existsb_exists.
+            esplits; [apply Ha|apply String.eqb_eq]; eauto.
+          * revert Ha2; unfold_mod; intros Ha2.
+            rr in Ha2; des; ss; subst.
+            unfold mn; rewrite !strings_maxlen_app; s.
+            rewrite mname_long_length; nia.
     }
     rewrite !CFilter.filter_app.
     
@@ -167,51 +151,56 @@ Section Helping.
 
     etrans; cycle 1.
     {
-      eapply ctxr_refines.
-      ctxr_rotate. ctxr_drop. ctxr_swap.
-      eapply MAIN; et.
+      eapply ctxr_refines. ctxr_norm.
+      do 2 ctxr_rotate. ctxr_drop. ctxr_drop. ctxr_swap. ctxr_swap.
+      eapply Hc1; et.
     }
 
     etrans; cycle 1.
     {
       eapply ctxr_refines.
-      do 2 ctxr_drop.
+      do 3 ctxr_drop.
       eapply helping_onoff_correct; et.
     }
 
     etrans; cycle 1.
     {
       eapply ctxr_refines.
-      ctxr_drop.
-      eapply CANCEL; et.
+      ctxr_drop. rewrite /mod_off. ctxr_drop.
+      eapply Hc2; et.
     }
 
     etrans; cycle 1.
     {
       eapply ctxr_refines.
-      do 2 ctxr_rotate. do 3 ctxr_drop. eapply CFilter.intro_filter.
+      ctxr_drop. ctxr_rotate. ctxr_drop. ctxr_drop.
+      apply CFilter.elim_module.
     }
+    rewrite -mod_add_empty_r.
 
     etrans; cycle 1.
     {
       eapply ctxr_refines.
-      ctxr_rotate. do 3 ctxr_drop. eapply CFilter.intro_filter.
+      do 2 ctxr_rotate. do 2 ctxr_drop. eapply CFilter.intro_filter.
     }
 
     etrans; cycle 1.
     { eapply ctxr_refines. do 2 ctxr_rotate. ctxr_refl. }
-    
+
     erewrite <-!CFilter.filter_app.
     etrans; [|eapply CFilter.elim_filter]; cycle 1.
-    { i. unfold mask, wmask_list. eapply existsb_exists.
-      esplits; [|eapply String.eqb_eq]; et.
-      eapply in_or_app; right.
-      eapply in_or_app; et.
+    {
+      intros fn Hin; eapply existsb_exists.
+      exists fn; split; last apply String.eqb_refl.
+      apply in_or_app; right.
+      apply in_or_app; left.
+      rewrite /md_src /Mod.exports.
+      apply elem_of_list_In, elem_of_list_omap; exists (Some fn); split; ss.
+      apply elem_of_list_In; eauto.
     }
 
     eapply ctxr_refines.
     eapply ctxr_cond_strengthen.
     iIntros "[[P1 P2] P]". iFrame.
   Qed.
-
-End Helping.   *)
+End Helping.  
